Core/Freshness.v
@@ -18,10 +18,11 @@ Lemma keys_last_mono f1 f2 k :
         (forall x, x \in dom f1 -> x \in dom f2) ->
         oleq (last k (dom f1)) (last k (dom f2)).
 Proof.
-rewrite !umEX; case: (UMC.from f1); first by move=>_ H _; apply: path_last H.
+rewrite !umEX; case: (UMC.from f1).
+- by move=>_ H _; apply: path_lastR H=>//; apply: otrans.
 move=>{f1} f1 /= _ H1; case: (UMC.from f2)=>/=.
 - by move=>_ /allP; case: (supp f1)=>//; rewrite /oleq eq_refl orbT.
-by move=>{f2} f2 /= _; apply: seq_last_mono H1.
+by move=>{f2} f2 /= _; apply: seq_last_monoR H1=>//; apply: otrans.
 Qed.
 
 End Keys.
@@ -48,14 +49,14 @@ rewrite /UM.empty UMC.eqE UM.umapE /supp fmapE /= {H H1}.
 by elim: s.
 Qed.
 
-Lemma dom_last_key f :  valid f -> ~~ empb f -> last_key f \in dom f.
-Proof. by move=>X; apply: contraR; move/(last_key_dom X)=>->; apply/empbP. Qed.
+Lemma dom_last_key f :  valid f -> ~~ unitb f -> last_key f \in dom f.
+Proof. by move=>X; apply: contraR; move/(last_key_dom X)=>->; apply: unitb0. Qed.
 
 Lemma last_key_max f x : x \in dom f -> x <= last_key f.
 Proof.
 rewrite /last_key /= !umEX; case: (UMC.from f)=>//; case=>s H _ /=.
 rewrite /supp /ord /= (leq_eqVlt x) orbC.
-by apply: sorted_last_key_max (sorted_oleq H).
+by apply: sorted_last_key_maxR (sorted_oleq H)=>//; apply: otrans.
 Qed.
 
 Lemma max_key_last f x :
@@ -63,6 +64,8 @@ Lemma max_key_last f x :
 Proof.
 rewrite /last_key !umEX; case: (UMC.from f)=>//; case=>s H _ /=.
 move=>H1 /= H2; apply: sorted_max_key_last (sorted_oleq H) H1 _.
+- by apply: otrans.
+- by apply: oantisym.
 by move=>z /(H2 z); rewrite leq_eqVlt orbC.
 Qed.
 
