Examples/Querying/QueryHooked.v
@@ -9,6 +9,7 @@ From DiSeL
 Require Import SeqLib QueryProtocol NewStatePredicates Actions.
 From DiSeL
 Require Import Injection Process Always HoareTriples InferenceRules While.
+Obligation Tactic := Tactics.program_simpl.
 
 Section QueryHooked.
 
@@ -30,7 +31,7 @@ Hypothesis core_state_to_data_inj :
 (* The query hook extracts certain data from the the core protocol *)
 (* local state if it's present there. *)
 Definition query_hook : hook_type :=
-  fun hc hq ms to => 
+  fun hc hq ms to =>
     forall n rid d, ms = rid :: serialize d -> core_state_to_data n hc d.
 
 Definition query_hookz := (1, (plab pc), (plab pq, tresp)) \\-> query_hook.
@@ -52,26 +53,20 @@ Lemma W_complete : hook_complete W.
 Proof.
 move=>z lc ls t/=; rewrite domPt inE=>/eqP[]_<-<-_.
 rewrite !domUn !inE/= !domPt !inE !eqxx/= orbC.
-case/andP:W_valid=>->_.
-rewrite 3!andTb.
-rewrite inE.
-by apply/orP; left.
+by case/andP:W_valid=>->_; rewrite andTb.
 Qed.
 
 Lemma W_dom : dom W.1 =i [:: plab pc; lq].
 Proof.
-move=>z/=; rewrite domUn !inE/=; case/andP: W_valid=>->/=_. 
-rewrite !domPt !inE; rewrite -!(eq_sym z).
-rewrite /cond /= inE orbC.
-apply sym_eq.
-by rewrite orbC eq_sym.
+move=>z/=; rewrite domUn !inE/=; case/andP: W_valid=>->/=_.
+by rewrite !domPt !inE; rewrite -!(eq_sym z) orbC.
 Qed.
 
-Lemma eqW : 
+Lemma eqW :
   W = (plab pc \\-> pc, Unit) \+ (plab pq \\-> pq, Unit) \+ (Unit, query_hookz).
 Proof. by rewrite /PCM.join/=/W !unitL !unitR. Qed.
 
-Lemma eqW' : 
+Lemma eqW' :
   W = (plab pc \\-> pc, Unit) \+ ((plab pq \\-> pq, Unit) \+ (Unit, query_hookz)).
 Proof. by rewrite eqW joinA. Qed.
 
@@ -79,17 +74,14 @@ Lemma injW : injects (plab pc \\-> pc, Unit) W query_hookz.
 Proof.
 rewrite eqW; apply:injectL=>//; try by move=>????/=; rewrite dom0 inE.
 - by rewrite -eqW W_valid.
-- move=>z lc ls t; rewrite domPt inE.
-  by rewrite /cond /= dom0.
-- move=>z lc ls t; rewrite domPt inE.
-  by rewrite /cond /= dom0.
+- by move=>z lc ls t; rewrite domPt inE dom0.
+- by move=>z lc ls t; rewrite domPt inE dom0.
 - move=>z lc ls t; rewrite domPt inE.
   case/eqP=>Z1 Z2 Z3 Z4; subst ls z lc t.
   rewrite !domUn !inE !domPt !inE !eqxx/=.
-  case/andP:W_valid=>/=->_/=; rewrite orbC inE.
-  by apply/orP; left.
+  by case/andP:W_valid=>/=->_/=; rewrite orbC.
 move=>l; rewrite domPt inE=>/eqP=><-.
-move=>z lc ls t; rewrite domPt inE=>/eqP[]_ _<-_.  
+move=>z lc ls t; rewrite domPt inE=>/eqP[]_ _<-_.
 apply/negbT; apply/eqP=>Z; subst lq; move/negbTE: Lab_neq.
 by rewrite eqxx.
 Qed.
@@ -102,17 +94,16 @@ Qed.
 
 Lemma labQ : lq \in dom W.1.
 Proof.
-case/andP: W_valid=>V1 V2.
-rewrite domUn !inE V1/= !domPt !inE /cond /= inE.
-by apply/orP; right.
+case/andP: W_valid=>V1 _.
+by rewrite domUn !inE V1/= !domPt !inE eq_refl orbC.
 Qed.
 
 Lemma injWQ : inj_ext injW = (lq \\-> pq, Unit).
 Proof.
 move: (W_valid)=>V; move: (cohK injW).
-rewrite {1}eqW/mkWorld/= -!joinA /PCM.join/= in V.
+rewrite {1}eqW/mkWorld/= -!joinA in V.
 case/andP: V=>/=V V'.
-rewrite {1}eqW/mkWorld/= -!joinA /PCM.join/=; case=>H K.
+rewrite {1}eqW/mkWorld/= -!joinA; case=>H K.
 case: (cancel V H)=>_; rewrite !unitR=>_{H}H1.
 rewrite [inj_ext _]surjective_pairing -H1{H1}; congr (_, _).
 rewrite !unitL joinC/=/query_hookz/= in V' K.
@@ -171,7 +162,7 @@ Definition query_init_state (to : nid) s :=
   [/\ to \in qnodes,
       holds_res_perms (getSq s) to (fun _ : nat => false),
       no_msg_from_to' this to request_msg (dsoup (getSq s)) &
-      no_msg_from_to' to this response_msg (dsoup (getSq s))].    
+      no_msg_from_to' to this response_msg (dsoup (getSq s))].
 
 (* This is the first serious one. *)
 Lemma query_init_step' z to s s' :
@@ -198,17 +189,17 @@ have Cq: coh pq (getStatelet s lq) by move: (coh_coh lq C1); rewrite /getProtoco
     rewrite domPt inE=>/eqP<-{m}; rewrite findPt; case=>_ _ Z; subst z.
     by rewrite eqxx in B.
   move/eqP: B=>B; subst z; split=>//; first 1 last.
-  + move=>m t c; rewrite findUnR ?valid_fresh ?(cohVs Cq)//; case: ifP; last by move=>_/G3.  
+  + move=>m t c; rewrite findUnR ?valid_fresh ?(cohVs Cq)//; case: ifP; last by move=>_/G3.
     rewrite domPt inE=>/eqP<-{m}; rewrite findPt; case=>_ _ Z; subst to.
     by move/negbTE: N; rewrite eqxx.
-  (* Now two interesting assertions. *)  
+  (* Now two interesting assertions. *)
   + move=>m t c; rewrite findUnR ?valid_fresh ?(cohVs Cq)//; case: ifP; last by move=>_/G4.
     rewrite domPt inE=>/eqP<-{m}; rewrite findPt; case=>Z' Z2 Z; subst to' t c.
     (* Consider two possible send-transitions. *)
-    case: H1;[|case=>//]; move=>Z; subst st=>//. 
+    case: H1;[|case=>//]; move=>Z; subst st=>//.
     case: (H4)=>_[C']/=[rid][d][_]; case: G2=>rq[rs][E]H.
     by rewrite (getStK _ E)/==>/H.
-  rewrite (cohVl Cq); case: G2=>rq[rs][E]H.  
+  rewrite (cohVl Cq); case: G2=>rq[rs][E]H.
   case: H1;[|case=>//]; move=>Z; subst st=>//; last first.
   + case: (H4)=>_[C']/=[rid][d][H']; subst msg.
     rewrite (getStK _ E)/==>G.
@@ -216,7 +207,7 @@ have Cq: coh pq (getStatelet s lq) by move: (coh_coh lq C1); rewrite /getProtoco
     subst n; eexists rq, (seq.rem (to', rid) rs); split=>//.
     by move=>rn; move/mem_rem; apply/H.
   case: (H4)=>_[C']/==>Z.
-  rewrite/QueryProtocol.send_req_prec (getStK _ E) in Z; subst msg. 
+  rewrite/QueryProtocol.send_req_prec (getStK _ E) in Z; subst msg.
   rewrite /=/QueryProtocol.send_step/=!(getStK _ E)/= in H6; case: H6=>Z; subst n.
   by exists ((to', fresh_id rq) :: rq), rs.
 (* Receive-transitions *)
@@ -226,13 +217,13 @@ rewrite /get_rt prEqQ'/==>Cq'; rewrite !(pf_irr Cq' Cq)=>{Cq'}.
 move=>rt pf H1 H2.
 case B: (to == z); rewrite /holds_res_perms/getLocal findU B/=; last first.
 - by split=>//; apply: no_msg_from_to_consume'=>//; rewrite ?(cohVs Cq).
-rewrite !(cohVl Cq); move/eqP:B=>B; subst z. 
+rewrite !(cohVl Cq); move/eqP:B=>B; subst z.
 split=>//; try by apply: no_msg_from_to_consume'=>//; rewrite ?(cohVs Cq).
 case: G2=>rq[rs][E]H.
 case: H1;[|case=>//]; move=>Z; subst rt=>//=; simpl in H2;
 rewrite /QueryProtocol.receive_step (getStK _ E)/=; last first.
 - case: ifP=>_; last by eexists _, _.
-  by exists (seq.rem (from, head 0 msg) rq), rs. 
+  by exists (seq.rem (from, head 0 msg) rq), rs.
 case: ifP=>_; last by eexists _, _.
 exists rq, ((from, head 0 msg) :: rs); split=>//.
 move=>rn; rewrite inE; case/orP; last by apply: H.
@@ -280,8 +271,8 @@ Qed.
 (* 1. We've just sent our stuff. *)
 Definition msg_just_sent d (reqs resp : seq (nid * nat)) req_num to :=
   [/\ getLocal this d = qst :-> (reqs, resp),
-   no_msg_from_to' to this response_msg (dsoup d), 
-   (to, req_num) \in reqs, 
+   no_msg_from_to' to this response_msg (dsoup d),
+   (to, req_num) \in reqs,
    msg_spec' this to treq ([:: req_num]) (dsoup d) &
    holds_res_perms d to (fun _ => false)].
 
@@ -301,7 +292,7 @@ Definition msg_responded d (reqs resp : seq (nid * nat)) req_num to data :=
    msg_spec' to this tresp (req_num :: serialize data) (dsoup d) &
    holds_res_perms d to (fun _ => false)].
 
-(* 4. Stability of the local state of a core protocol, 
+(* 4. Stability of the local state of a core protocol,
       to be proved separately *)
 
 (* A local assertion ensuring stability of the core_state_to_data *)
@@ -311,19 +302,19 @@ Hypothesis core_state_stable_step : forall z s data s' n,
   this != z -> network_step (plab pc \\-> pc, Unit) z s s' ->
   n \in qnodes ->
   local_indicator data (getLc s) ->
-  core_state_to_data n (getLc' s n) data  -> 
+  core_state_to_data n (getLc' s n) data  ->
   core_state_to_data n (getLc' s' n) data.
 
 Lemma prEqC' : (getProtocol (plab pc \\-> pc, Unit) (plab pc)) = pc.
 Proof. by rewrite /getProtocol findPt/=. Qed.
-  
+
 (* Showing that the core assertion is stable *)
 Lemma core_state_stable_step_W s data s' z :
   this != z ->
   network_step W z s s' ->
   z \in qnodes ->
   local_indicator data (getLc s) ->
-  core_state_to_data z (getLc' s z) data -> 
+  core_state_to_data z (getLc' s z) data ->
   core_state_to_data z (getLc' s' z) data.
 Proof.
 move=>N H2 G L H1; move:(step_coh H2)=>[C1 C2].
@@ -337,7 +328,7 @@ move: (C1) (C2) =>C1' C2'.
 rewrite E1 E2 in H2 C1' C2'.
 have [X X'] : (forall z, getLc' s z  = getLc' s1 z) /\
               (forall z, getLc' s' z = getLc' s1' z).
-- by split; move=>z'; rewrite /getStatelet find_umfilt domPt inE eqxx.
+- by split; move=>z'; rewrite /getStatelet find_umfiltk domPt inE eqxx.
 case: (sem_split injW _ _ H2).
 - apply: (@projectS_cohL (plab pc \\-> pc, Unit)
                          ((plab pq \\-> pq, Unit) \+ (Unit, query_hookz)))=>//.
@@ -354,7 +345,7 @@ Lemma core_state_stable s data s' z :
   network_rely W this s s' ->
   z \in qnodes ->
   local_indicator data (getLc s) ->
-  core_state_to_data z (getLc' s z) data -> 
+  core_state_to_data z (getLc' s z) data ->
   core_state_to_data z (getLc' s' z) data.
 Proof.
 move=> R Z L. move: (L); rewrite -(@rely_loc' _ _ (plab pc) s s' R)=>L'.
@@ -363,7 +354,7 @@ case B: (this == z); [move/eqP: B=>B|move/negbT: B=>B].
 - by subst z=>R; rewrite (@rely_loc' _ _ (plab pc) s s' R).
 move=>[n]H2 H1; elim: n s H2=>/=[s | n Hi s]; first by case=>Z _; subst s'.
 case=>y[s1][N]G1 G2 G3 G4; apply: (Hi s1 G2).
-- by rewrite /getLocal -(step_is_local (plab pc) G1 N). 
+- by rewrite /getLocal -(step_is_local (plab pc) G1 N).
 case B' : (z == y); [move/eqP: B'=>B' | move/negbT: B'=>B'].
 - by subst y; apply: (core_state_stable_step_W _ _ _ _ B G1 _ G3).
 by rewrite /getLocal -(step_is_local (plab pc) G1 B').
@@ -377,14 +368,14 @@ Lemma cohQ s : Coh W s -> (QueryProtocol.QCoh qnodes) (getSq s).
 Proof. by move/(coh_coh lq); rewrite prEqQ. Qed.
 
 Lemma send_lq_case1 req_num reqs resp to s
-  (N : this != to) (Qn : to \in qnodes) 
+  (N : this != to) (Qn : to \in qnodes)
   (M : msg_just_sent (getSq s) reqs resp req_num to)
   to' msg (n : heap) (C : Coh W s) (st : send_trans (Protocols.coh pq))
   (H1 : st \In snd_trans pq)
   (H2 : to \in qnodes)
-  (H4 : send_safe st to to' (getSq s) msg) : 
+  (H4 : send_safe st to to' (getSq s) msg) :
   all_hooks_fire query_hookz (plab pq) (t_snd st) s to msg to' -> Some n = send_step H4 ->
-  let: d := getStatelet (upd (plab pq) 
+  let: d := getStatelet (upd (plab pq)
               (DStatelet (upd to n (dstate (getSq s)))
                (dsoup (getSq s) \+ fresh (dsoup (getSq s)) \\->
                       Msg (TMsg (t_snd st) msg) to to' true)) s) lq in
@@ -397,24 +388,24 @@ move=>H5 H6; case: M=>G1 G2 G3 G4[rq][rs][E]Np; split=>//.
   case: ifP; [|by move=>_; apply: G2].
   rewrite domPt inE=>/eqP<-; rewrite findPt; case=>???; subst t c to'.
   case: H1;[|case=>//]; move=>Z; subst st=>//; simpl in H5, H6;
-  rewrite/QueryProtocol.send_step (getStK _ E)/= in H6; case: H6=>H6/=; subst n.                                  
-  by case:H4=>_[C'][rid][_][_]; rewrite (getStK _ E); move/Np. 
+  rewrite/QueryProtocol.send_step (getStK _ E)/= in H6; case: H6=>H6/=; subst n.
+  by case:H4=>_[C'][rid][_][_]; rewrite (getStK _ E); move/Np.
 - rewrite /getStatelet findU  eqxx(cohS C)/=.
   case:G4; case=>i[[c']Q1 Q3] Q2; split; last first.
   + move=>j c; rewrite findUnR ?(valid_fresh) ?(cohVs (cohQ s C))//.
-    case:ifP; last by move=>_; apply Q2. 
+    case:ifP; last by move=>_; apply Q2.
     rewrite domPt inE=>/eqP<-; rewrite findPt.
     by case=>???; subst to; rewrite eqxx in N.
-  exists i; split=>[|j[c1]];rewrite findUnL ?(valid_fresh) ?(cohVs (cohQ s C))//.   
-  + by exists c'; rewrite (find_some Q1). 
-  case: ifP=>_; first by move=> T; apply: Q3; exists c1. 
-  by case/findPt_inv=>_[]_ _?; subst to; rewrite eqxx in N. 
+  exists i; split=>[|j[c1]];rewrite findUnL ?(valid_fresh) ?(cohVs (cohQ s C))//.
+  + by exists c'; rewrite (find_some Q1).
+  case: ifP=>_; first by move=> T; apply: Q3; exists c1.
+  by case/findPt_inv=>_[]_ _?; subst to; rewrite eqxx in N.
 rewrite /getStatelet findU eqxx (cohS C)/=/holds_res_perms.
-rewrite /getLocal/=findU eqxx/= (cohVl (cohQ s C)).  
+rewrite /getLocal/=findU eqxx/= (cohVl (cohQ s C)).
 case: H1;[|case=>//]; move=>Z; subst st=>//; simpl in H5, H6;
 rewrite/QueryProtocol.send_step (getStK _ E)/= in H6; case: H6=>H6; subst n.
 - by exists ((to', fresh_id rq) :: rq), rs.
-case: ifP=>_; last by exists rq, rs.                 
+case: ifP=>_; last by exists rq, rs.
 by exists rq, (seq.rem (to', head 0 msg) rs); split=>//rn/mem_rem/Np.
 Qed.
 
@@ -425,13 +416,13 @@ Lemma send_lq_case3 req_num data reqs resp to s
   to' msg (n : heap) (C : Coh W s) (st : send_trans (Protocols.coh pq))
   (H1 : st \In snd_trans pq)
   (H2 : to \in qnodes)
-  (H4 : send_safe st to to' (getSq s) msg) : 
+  (H4 : send_safe st to to' (getSq s) msg) :
   all_hooks_fire query_hookz (plab pq) (t_snd st) s to msg to' -> Some n = send_step H4 ->
-  let: d := getStatelet (upd (plab pq) 
+  let: d := getStatelet (upd (plab pq)
               (DStatelet (upd to n (dstate (getSq s)))
                (dsoup (getSq s) \+ fresh (dsoup (getSq s)) \\->
                       Msg (TMsg (t_snd st) msg) to to' true)) s) lq in
-  msg_responded d reqs resp req_num to data.  
+  msg_responded d reqs resp req_num to data.
 Proof.
 move=>H5 H6.
 case: M=>G1 G2 G3 G4[rq][rs][E]Np; split=>//.
@@ -444,25 +435,25 @@ case: M=>G1 G2 G3 G4[rq][rs][E]Np; split=>//.
 - rewrite /getStatelet findU  eqxx(cohS C)/=.
   case:G4; case=>i[[c']Q1 Q3] Q2; split; last first.
   + move=>j c; rewrite findUnR ?(valid_fresh) ?(cohVs (cohQ s C))//.
-    case:ifP; last by move=>_; apply Q2. 
+    case:ifP; last by move=>_; apply Q2.
     rewrite domPt inE=>/eqP<-; rewrite findPt.
     case=>???; subst to' c.
     case: H1;[|case=>//]; move=>Z; subst st=>//; simpl in H5, H6;
     rewrite/QueryProtocol.send_step (getStK _ E)/= in H6; case: H6=>H6/=; subst n.
-    by case:H4=>_[C']; rewrite (getStK _ E); case=>rid[d][->]/=/Np. 
-  exists i; split=>[|j[c1]];rewrite findUnL ?(valid_fresh) ?(cohVs (cohQ s C))//.   
-  + by exists c'; rewrite (find_some Q1). 
-  case: ifP=>_; first by move=> T; apply: Q3; exists c1. 
+    by case:H4=>_[C']; rewrite (getStK _ E); case=>rid[d][->]/=/Np.
+  exists i; split=>[|j[c1]];rewrite findUnL ?(valid_fresh) ?(cohVs (cohQ s C))//.
+  + by exists c'; rewrite (find_some Q1).
+  case: ifP=>_; first by move=> T; apply: Q3; exists c1.
   case/findPt_inv=>_[]???; subst to'.
   case: H1;[|case=>//]; move=>Z; subst st=>//; simpl in H5, H6;
   rewrite/QueryProtocol.send_step (getStK _ E)/= in H6; case: H6=>H6/=; subst n.
-  by case:H4=>_[C']; rewrite (getStK _ E); case=>rid[d][_]/=/Np. 
+  by case:H4=>_[C']; rewrite (getStK _ E); case=>rid[d][_]/=/Np.
 rewrite /getStatelet findU eqxx (cohS C)/=/holds_res_perms.
-rewrite /getLocal/=findU eqxx/= (cohVl (cohQ s C)).  
+rewrite /getLocal/=findU eqxx/= (cohVl (cohQ s C)).
 case: H1;[|case=>//]; move=>Z; subst st=>//; simpl in H5, H6;
 rewrite/QueryProtocol.send_step (getStK _ E)/= in H6; case: H6=>H6; subst n.
 - by exists ((to', fresh_id rq) :: rq), rs.
-case: ifP=>_; last by exists rq, rs.                 
+case: ifP=>_; last by exists rq, rs.
 by exists rq, (seq.rem (to', head 0 msg) rs); split=>//rn/mem_rem/Np.
 Qed.
 
@@ -474,36 +465,36 @@ Lemma send_lq_all_cases req_num data reqs resp to s
   to' msg (n : heap) (C : Coh W s) (st : send_trans (Protocols.coh (getProtocol W (plab pq))))
   (H1 : st \In get_st W (plab pq))
   (H2 : to \in nodes (getProtocol W (plab pq)) (getSq s))
-  (H4 : send_safe st to to' (getSq s) msg) : 
+  (H4 : send_safe st to to' (getSq s) msg) :
   all_hooks_fire query_hookz (plab pq) (t_snd st) s to msg to' -> Some n = send_step H4 ->
-  let: d := getStatelet (upd (plab pq) 
+  let: d := getStatelet (upd (plab pq)
               (DStatelet (upd to n (dstate (getSq s)))
                (dsoup (getSq s) \+ fresh (dsoup (getSq s)) \\->
                       Msg (TMsg (t_snd st) msg) to to' true)) s) lq in
   [\/ msg_just_sent d reqs resp req_num to,
       msg_received  d reqs resp req_num to
-    | msg_responded d reqs resp req_num to data].  
+    | msg_responded d reqs resp req_num to data].
 Proof.
 move=>H5 H6.
 move: st H1 H4 H5 H6; rewrite /get_st prEqQ=>st H1 H4 H5 H6.
 case: M; last 1 first.
 + (* already responded to our request, should be boring *)
   constructor 3.
-  by apply: (send_lq_case3 req_num data  _ _ _ _ _ _ _ _ _ _ _ _ _ _ _ _ H4). 
+  by apply: (send_lq_case3 req_num data  _ _ _ _ _ _ _ _ _ _ _ _ _ _ _ _ H4).
 + (* just sent the request *)
-  by constructor 1; apply: (send_lq_case1 req_num _ _ _ _ _ _ _ _ _ _ _ _ _ _ H4). 
+  by constructor 1; apply: (send_lq_case1 req_num _ _ _ _ _ _ _ _ _ _ _ _ _ _ H4).
 
 Ltac kill_g3 s C G3 to N :=
   rewrite /getStatelet findU  eqxx(cohS C)/==>z t c;
   rewrite findUnR ?(valid_fresh) ?(cohVs (cohQ s C))//;
-  case: ifP; [|by move=>_; apply: G3]; 
+  case: ifP; [|by move=>_; apply: G3];
   rewrite domPt inE=>/eqP<-; rewrite findPt;
   by case=>_ _ Z _; subst to; rewrite eqxx in N.
 
 Ltac kill_g4 s C G4 to' t B:=
   rewrite /getStatelet findU  eqxx(cohS C)/==>z t c;
   rewrite findUnR ?(valid_fresh) ?(cohVs (cohQ s C))//;
-  case: ifP; [|by move=>_; apply: G4]; 
+  case: ifP; [|by move=>_; apply: G4];
   rewrite domPt inE=>/eqP<-; rewrite findPt;
   by case=>??; try move=>?; try subst t; try subst to'; try rewrite ?eqxx in B.
 
@@ -512,27 +503,27 @@ case=>G1 G2 G3 G4 [rq][rs][E]Np.
 case B : (to' == this); [move/eqP:B=>B; subst to'|]; last first.
 - constructor 2. (* boring case : sending to someone else*)
   split=>//.
-  + by rewrite /getStatelet findU eqxx(cohS C)/=/getLocal/= findU (negbTE N) in G1 *. 
-  + kill_g3 s C G3 to N.
-  + kill_g4 s C G4 to' t B.
-  rewrite /getStatelet findU eqxx (cohS C)/=/holds_res_perms.
-  rewrite /getLocal/=findU eqxx/= (cohVl (cohQ s C)).  
-  case: H1;[|case=>//]; move=>Z; subst st=>//; simpl in H5, H6;
-  rewrite/QueryProtocol.send_step (getStK _ E)/= in H6; case: H6=>H6; subst n.
-  - by exists ((to', fresh_id rq) :: rq), rs. 
-  case:ifP=>_; last by exists rq, rs.   
-  by exists rq, (seq.rem (to', head 0 msg) rs); split=>//rn/mem_rem/Np.
-(* Actually sending to us. *)  
-case: H1;[|case=>//]; move=>Z; subst st=>//; simpl in H5, H6;
-rewrite/QueryProtocol.send_step (getStK _ E)/= in H6; case: H6=>H6; subst n.                                  
-- constructor 2; split=>//. (* sending request (not response) -- this is boring *)
-  + by rewrite /getStatelet findU eqxx(cohS C)/=/getLocal/= findU (negbTE N) in G1 *. 
+  + by rewrite /getStatelet findU eqxx(cohS C)/=/getLocal/= findU (negbTE N) in G1 *.
   + kill_g3 s C G3 to N.
   + kill_g4 s C G4 to' t B.
   rewrite /getStatelet findU eqxx (cohS C)/=/holds_res_perms.
   rewrite /getLocal/=findU eqxx/= (cohVl (cohQ s C)).
-  by exists ((this, fresh_id rq) :: rq), rs.    
-(* Sending response to us!!! *)                                          
+  case: H1;[|case=>//]; move=>Z; subst st=>//; simpl in H5, H6;
+  rewrite/QueryProtocol.send_step (getStK _ E)/= in H6; case: H6=>H6; subst n.
+  - by exists ((to', fresh_id rq) :: rq), rs.
+  case:ifP=>_; last by exists rq, rs.
+  by exists rq, (seq.rem (to', head 0 msg) rs); split=>//rn/mem_rem/Np.
+(* Actually sending to us. *)
+case: H1;[|case=>//]; move=>Z; subst st=>//; simpl in H5, H6;
+rewrite/QueryProtocol.send_step (getStK _ E)/= in H6; case: H6=>H6; subst n.
+- constructor 2; split=>//. (* sending request (not response) -- this is boring *)
+  + by rewrite /getStatelet findU eqxx(cohS C)/=/getLocal/= findU (negbTE N) in G1 *.
+  + kill_g3 s C G3 to N.
+  + kill_g4 s C G4 to' t B.
+  rewrite /getStatelet findU eqxx (cohS C)/=/holds_res_perms.
+  rewrite /getLocal/=findU eqxx/= (cohVl (cohQ s C)).
+  by exists ((this, fresh_id rq) :: rq), rs.
+(* Sending response to us!!! *)
 case: (H4)=>_[C']/=[rid][d][Zm]Tr; subst msg.
 rewrite  (getStK _ E)/= in Tr.
 rewrite Tr; constructor 3.
@@ -546,27 +537,27 @@ split=>//; first 3 last.
   rewrite /getLocal findU eqxx/= (cohVl C'); split=>// rn R.
   move/Np/eqP: (mem_rem R)=>Zr; subst rn.
   move/Np:Tr=>/eqP=>Zr; subst rid.
-  case: (C')=>_ _ _/(_ to); rewrite E (cohDom C')=>/(_ Qn). 
+  case: (C')=>_ _ _/(_ to); rewrite E (cohDom C')=>/(_ Qn).
   case=>[[x1 x2]][]/(hcancelPtV _); rewrite validPt/==>/(_ is_true_true).
   case=>Z1 Z2; subst x1 x2=>/andP[_]G.
   by rewrite (rem_filter (this, req_num) G) mem_filter/= eqxx/= in R.
-+ by rewrite /getStatelet findU eqxx(cohS C)/getLocal findU (negbTE N). 
++ by rewrite /getStatelet findU eqxx(cohS C)/getLocal findU (negbTE N).
 + rewrite /getStatelet findU eqxx (cohS C)/==>z t c.
   rewrite findUnR ?(valid_fresh) ?(cohVs C')//.
   case: ifP=>[|_]; last by apply: G3.
   by rewrite domPt inE=>/eqP<-{z}; rewrite findPt; case=><-.
-(* Here's the big hooking moment *)  
-split=>[|i m]; 
+(* Here's the big hooking moment *)
+split=>[|i m];
   rewrite /getStatelet findU eqxx/= (cohS C)/=; last first.
-+ rewrite findUnR ?(valid_fresh) ?(cohVs C')//; case: ifP=>[|_]; last by move/G4. 
++ rewrite findUnR ?(valid_fresh) ?(cohVs C')//; case: ifP=>[|_]; last by move/G4.
   rewrite domPt inE=>/eqP<-; rewrite findPt; case=><-.
   by move/Np/eqP: Tr=>->; rewrite eqxx.
 exists (fresh (dsoup (getStatelet s lq))); split.
 + exists (rid :: serialize data).
   by rewrite findUnR ?(valid_fresh)?(cohVs C')// domPt inE eqxx findPt.
 move=>i[c]; rewrite findUnR ?(valid_fresh)?(cohVs C')//.
-case: ifP=>[|_]; last by move/G4. 
-by rewrite domPt inE=>/eqP<-; rewrite findPt. 
+case: ifP=>[|_]; last by move/G4.
+by rewrite domPt inE=>/eqP<-; rewrite findPt.
 Qed.
 
 (*  A lemma covering send-cases in the lc-part of the world  *)
@@ -578,20 +569,20 @@ Lemma send_lc_all_cases req_num data reqs resp to s
   to' msg (n : heap) (C : Coh W s) (st : send_trans (Protocols.coh (getProtocol W (plab pc))))
   (H1 : st \In get_st W (plab pc))
   (H2 : to \in nodes (getProtocol W (plab pc)) (getSq s))
-  (H4 : send_safe st to to' (getSq s) msg) : 
+  (H4 : send_safe st to to' (getSq s) msg) :
   all_hooks_fire query_hookz (plab pc) (t_snd st) s to msg to' -> Some n = send_step H4 ->
-  let: d := getStatelet (upd (plab pc) 
+  let: d := getStatelet (upd (plab pc)
               (DStatelet (upd to n (dstate (getSq s)))
                (dsoup (getSq s) \+ fresh (dsoup (getSq s)) \\->
                       Msg (TMsg (t_snd st) msg) to to' true)) s) lq in
   [\/ msg_just_sent d reqs resp req_num to,
       msg_received  d reqs resp req_num to
-    | msg_responded d reqs resp req_num to data].  
+    | msg_responded d reqs resp req_num to data].
 Proof.
 move=>H5 H6.
 move: st H1 H4 H5 H6; rewrite /get_st prEqC=>st H1 H4 H5 H6.
 by case: M; [constructor 1|constructor 2|constructor 3];
-   rewrite /getStatelet findU (negbTE Lab_neq)/=. 
+   rewrite /getStatelet findU (negbTE Lab_neq)/=.
 Qed.
 
 Lemma recv_lq_case1 req_num reqs resp to s
@@ -599,56 +590,56 @@ Lemma recv_lq_case1 req_num reqs resp to s
   (M : msg_just_sent (getSq s) reqs resp req_num to)
   i from msg (C : Coh W s) (C' : (coh pq) (getSq s))
   (pf : to \in nodes pq (getSq s))
-  (rt : receive_trans (Protocols.coh pq)) : 
+  (rt : receive_trans (Protocols.coh pq)) :
   rt \In rcv_trans pq -> tag msg = t_rcv rt ->
   find i (dsoup (getSq s)) = Some (Msg msg from to true) ->
-  let: d := getStatelet (upd (plab pq) 
+  let: d := getStatelet (upd (plab pq)
               (DStatelet (upd to (receive_step rt from msg C' pf) (dstate (getSq s)))
                (consume_msg (dsoup (getSq s)) i)) s) lq in
   msg_just_sent d reqs resp req_num to \/
-  msg_received d reqs resp req_num to. 
+  msg_received d reqs resp req_num to.
 Proof.
 move=>H1 H2 H4; case: M=>G1 G2 G3 G4[rq][rs][Tr]Np.
 case X: (this == from); [move/eqP:X=>X; subst from|constructor 1];
 last first.
 - split=>//.
-  + by rewrite /getStatelet findU eqxx(cohS C)/=/getLocal/= findU (negbTE N) in G1 *. 
+  + by rewrite /getStatelet findU eqxx(cohS C)/=/getLocal/= findU (negbTE N) in G1 *.
   + rewrite /getStatelet findU eqxx(cohS C)/=.
     by apply: no_msg_from_to_consume'=>//; rewrite (cohVs C').
   + rewrite /getStatelet findU eqxx(cohS C)/=.
     case: msg H2 H4=>t c H2 H4.
-    by apply: (msg_spec_consumeE (cohVs C') H4 G4); rewrite (negbT X).   
+    by apply: (msg_spec_consumeE (cohVs C') H4 G4); rewrite (negbT X).
   rewrite /getStatelet findU eqxx (cohS C)/=/holds_res_perms.
-  rewrite /getLocal/=findU eqxx/= (cohVl (cohQ s C)).  
+  rewrite /getLocal/=findU eqxx/= (cohVl (cohQ s C)).
   case: H1;[|case=>//]; move=>Z; subst rt=>//=; simpl in H2, H4;
   rewrite/QueryProtocol.receive_step (getStK _ Tr)/=.
-  + case:ifP=>_; last by exists rq, rs. 
+  + case:ifP=>_; last by exists rq, rs.
     exists rq, ((from, head 0 msg) :: rs); split=>//rn.
     by rewrite inE; case/orP; [case/eqP=>Z; subst; rewrite eqxx in X|move/Np].
-  case:ifP=>_; last by exists rq, rs. 
-  by exists (seq.rem (from, head 0 msg) rq), rs. 
+  case:ifP=>_; last by exists rq, rs.
+  by exists (seq.rem (from, head 0 msg) rq), rs.
 case: msg H2 H4=>t c H2 H4.
 case: H1;[|case=>//]; move=>Z; subst rt=>//=; simpl in H2, H4; subst t; last first.
 - constructor 1; split=>//.
-  + by rewrite /getStatelet findU eqxx(cohS C)/=/getLocal/= findU (negbTE N) in G1 *. 
+  + by rewrite /getStatelet findU eqxx(cohS C)/=/getLocal/= findU (negbTE N) in G1 *.
   + rewrite /getStatelet findU eqxx(cohS C)/=.
     by apply: no_msg_from_to_consume'=>//; rewrite (cohVs C').
   + rewrite /getStatelet findU eqxx(cohS C)/=.
     by apply: (msg_spec_consumeE (cohVs C') H4 G4)=>/=; rewrite -(orbC true)/= orbC.
   rewrite /getStatelet findU eqxx (cohS C)/=/holds_res_perms.
-  rewrite /getLocal/=findU eqxx/= (cohVl (cohQ s C)).  
+  rewrite /getLocal/=findU eqxx/= (cohVl (cohQ s C)).
   rewrite/QueryProtocol.receive_step (getStK _ Tr)/=.
-  case:ifP=>_; last by exists rq, rs. 
-  by exists (seq.rem (this, head 0 c) rq), rs.  
+  case:ifP=>_; last by exists rq, rs.
+  by exists (seq.rem (this, head 0 c) rq), rs.
 (* Finally, the only interesting case here *)
-constructor 2; split=>//.  
-+ by rewrite /getStatelet findU eqxx(cohS C)/=/getLocal/= findU (negbTE N) in G1 *.     
+constructor 2; split=>//.
++ by rewrite /getStatelet findU eqxx(cohS C)/=/getLocal/= findU (negbTE N) in G1 *.
 + rewrite /getStatelet findU eqxx(cohS C)/=.
   by apply: (no_msg_spec_consume (cohVs C') H4 G4).
 + rewrite /getStatelet findU eqxx(cohS C)/=.
   by apply: no_msg_from_to_consume'=>//; rewrite (cohVs C').
 rewrite /getStatelet findU eqxx (cohS C)/=/holds_res_perms.
-rewrite /getLocal/=findU eqxx/= (cohVl (cohQ s C)).  
+rewrite /getLocal/=findU eqxx/= (cohVl (cohQ s C)).
 rewrite/QueryProtocol.receive_step (getStK _ Tr)/=.
 case:ifP=>X; last by move/negbT/negbNE/Np: X.
 exists rq, ((this, head 0 c) :: rs); split=>//rn.
@@ -661,33 +652,33 @@ Lemma recv_lq_case2 req_num reqs resp to s
   (M : msg_received (getSq s) reqs resp req_num to)
   i from msg (C : Coh W s) (C' : (coh pq) (getSq s))
   (pf : to \in nodes pq (getSq s))
-  (rt : receive_trans (Protocols.coh pq)) : 
+  (rt : receive_trans (Protocols.coh pq)) :
   rt \In rcv_trans pq -> tag msg = t_rcv rt ->
   find i (dsoup (getSq s)) = Some (Msg msg from to true) ->
-  let: d := getStatelet (upd (plab pq) 
+  let: d := getStatelet (upd (plab pq)
               (DStatelet (upd to (receive_step rt from msg C' pf) (dstate (getSq s)))
                (consume_msg (dsoup (getSq s)) i)) s) lq in
-  msg_received d reqs resp req_num to.  
+  msg_received d reqs resp req_num to.
 Proof.
 move=>H1 H2 H4; case: M=>G1 G2 G3 G4[rq][rs][Tr]Np.
 split=>//.
-- by rewrite /getStatelet findU eqxx(cohS C)/=/getLocal/= findU (negbTE N) in G1 *. 
+- by rewrite /getStatelet findU eqxx(cohS C)/=/getLocal/= findU (negbTE N) in G1 *.
 - rewrite /getStatelet findU eqxx(cohS C)/=.
   by apply: no_msg_from_to_consume'=>//; rewrite (cohVs C').
-- rewrite /getStatelet findU eqxx(cohS C)/=.  
+- rewrite /getStatelet findU eqxx(cohS C)/=.
   by apply: no_msg_from_to_consume'=>//; rewrite (cohVs C').
 rewrite /getStatelet findU eqxx (cohS C)/=/holds_res_perms.
-rewrite /getLocal/=findU eqxx/= (cohVl (cohQ s C)).  
+rewrite /getLocal/=findU eqxx/= (cohVl (cohQ s C)).
 case: H1;[|case=>//]; move=>Z; subst rt=>//=; simpl in H2, H4;
 rewrite/QueryProtocol.receive_step (getStK _ Tr)/=.
-- case:ifP=>_; last by exists rq, rs. 
+- case:ifP=>_; last by exists rq, rs.
   exists rq, ((from, head 0 msg) :: rs); split=>//rn.
   case X: (this == from); last first.
   + by rewrite inE; case/orP; [case/eqP=>Z; subst; rewrite eqxx in X|move/Np].
   move/eqP:X=>X; subst from.
-  by case: msg H2 H4=>t c/= H2 H4; move: (G3 _ _ _ H4); subst t.  
-case:ifP=>_; last by exists rq, rs. 
-by exists (seq.rem (from, head 0 msg) rq), rs. 
+  by case: msg H2 H4=>t c/= H2 H4; move: (G3 _ _ _ H4); subst t.
+case:ifP=>_; last by exists rq, rs.
+by exists (seq.rem (from, head 0 msg) rq), rs.
 Qed.
 
 Lemma recv_lq_case3 req_num reqs resp to s data
@@ -697,34 +688,34 @@ Lemma recv_lq_case3 req_num reqs resp to s data
   (L : local_indicator data (getLc' s this))
   i from msg (C : Coh W s) (C' : (coh pq) (getSq s))
   (pf : to \in nodes pq (getSq s))
-  (rt : receive_trans (Protocols.coh pq)) : 
+  (rt : receive_trans (Protocols.coh pq)) :
   rt \In rcv_trans pq -> tag msg = t_rcv rt ->
   find i (dsoup (getSq s)) = Some (Msg msg from to true) ->
-  let: d := getStatelet (upd (plab pq) 
+  let: d := getStatelet (upd (plab pq)
               (DStatelet (upd to (receive_step rt from msg C' pf) (dstate (getSq s)))
                (consume_msg (dsoup (getSq s)) i)) s) lq in
-  msg_responded d reqs resp req_num to data.  
+  msg_responded d reqs resp req_num to data.
 Proof.
 move=>H1 H2 H4; case: M=>G1 G2 G3 G4[rq][rs][Tr]Np.
 split=>//.
-- by rewrite /getStatelet findU eqxx(cohS C)/=/getLocal/= findU (negbTE N) in G1 *. 
+- by rewrite /getStatelet findU eqxx(cohS C)/=/getLocal/= findU (negbTE N) in G1 *.
 - rewrite /getStatelet findU eqxx(cohS C)/=.
   by apply: no_msg_from_to_consume'=>//; rewrite (cohVs C').
 - rewrite /getStatelet findU eqxx(cohS C)/=.
   case: msg H2 H4=>t c H2 H4.
   by apply: (msg_spec_consumeE (cohVs C') H4 G4); rewrite N orbC.
 rewrite /getStatelet findU eqxx (cohS C)/=/holds_res_perms.
-rewrite /getLocal/=findU eqxx/= (cohVl (cohQ s C)).  
+rewrite /getLocal/=findU eqxx/= (cohVl (cohQ s C)).
 case: H1;[|case=>//]; move=>Z; subst rt=>//=; simpl in H2, H4;
 rewrite/QueryProtocol.receive_step (getStK _ Tr)/=.
-- case:ifP=>_; last by exists rq, rs. 
+- case:ifP=>_; last by exists rq, rs.
   exists rq, ((from, head 0 msg) :: rs); split=>//rn.
   case X: (this == from); last first.
   + by rewrite inE; case/orP; [case/eqP=>Z; subst; rewrite eqxx in X|move/Np].
   move/eqP:X=>X; subst from.
-  by case: msg H2 H4=>t c/= H2 H4; move: (G3 _ _ _ H4); subst t.  
-case:ifP=>_; last by exists rq, rs. 
-by exists (seq.rem (from, head 0 msg) rq), rs. 
+  by case: msg H2 H4=>t c/= H2 H4; move: (G3 _ _ _ H4); subst t.
+case:ifP=>_; last by exists rq, rs.
+by exists (seq.rem (from, head 0 msg) rq), rs.
 Qed.
 
 (***********************************************************)
@@ -734,7 +725,7 @@ Qed.
 Definition msg_story s req_num to data reqs resp :=
   [/\ to \in qnodes,
      core_state_to_data to (getLc' s to) data,
-     local_indicator data (getLc s) & 
+     local_indicator data (getLc s) &
      let: d := getSq s in
      [\/ msg_just_sent d reqs resp req_num to,
       msg_received d reqs resp req_num to |
@@ -761,7 +752,7 @@ case: S; [by case=>_<- |
 (* Something sending in lc, should be irrelevant for us. *)
 - move: st H1 H4 H5 H6; rewrite /get_st prEqC=>st H1 H4 H5 H6.
   by case: M; [constructor 1|constructor 2|constructor 3];
-     rewrite /getStatelet findU (negbTE Lab_neq). 
+     rewrite /getStatelet findU (negbTE Lab_neq).
 
 (* Something sending in lq, this is where the interesting stuff happens! *)
 - by apply: send_lq_all_cases.
@@ -769,9 +760,9 @@ case: S; [by case=>_<- |
 (* Something is receiving in lc, should be irrelevant for us. *)
 - move: (coh_s _ _) rt pf H1 H2 H4; rewrite /get_rt prEqC=>C' rt pf H1 H2 H4.
   by case: M; [constructor 1|constructor 2|constructor 3];
-     rewrite /getStatelet findU (negbTE Lab_neq). 
+     rewrite /getStatelet findU (negbTE Lab_neq).
 
-(* Something receiving in lq, requires honest proving. *)  
+(* Something receiving in lq, requires honest proving. *)
 move: (coh_s _ _) rt pf H1 H2 H4; rewrite /get_rt prEqQ=>C' rt pf H1 H2 H4.
 case: M=>M;[|constructor 2|constructor 3]; last first.
 - by apply: recv_lq_case3.
@@ -799,7 +790,7 @@ case: S; [by case=>_<- |
   rewrite -(cohD C) domUn !inE !domPt !inE in H3;
   case/andP:H3=>_ H3; case/orP: H3=>/eqP H3; subst l;
   do? [by rewrite /getStatelet findU (negbTE Lab_neq)];
-  rewrite /getStatelet findU eqxx(cohS C)/=.                
+  rewrite /getStatelet findU eqxx(cohS C)/=.
 
 (* Now only consider send-receive transitions within pq protocol *)
 
@@ -807,9 +798,9 @@ case: S; [by case=>_<- |
 case:M; case=>G1 G2 G3 G4 G5; [constructor 1|constructor 2|constructor 3].
 
 (* Send-transition, case 1 *)
-- split=>//=; first by rewrite /getLocal/= findU (negbTE N) in G1 *. 
+- split=>//=; first by rewrite /getLocal/= findU (negbTE N) in G1 *.
   + move=>i t c; rewrite findUnR ?(valid_fresh) ?(cohVs (cohQ s C))//.
-    case:ifP; last by move=>_; apply G2. 
+    case:ifP; last by move=>_; apply G2.
     rewrite domPt inE=>/eqP<-; rewrite findPt.
     by case=>???; subst to; rewrite eqxx in A.
   + case: G4; case=>i[[c']Q1 Q3] Q2; split; last first.
@@ -817,28 +808,28 @@ case:M; case=>G1 G2 G3 G4 G5; [constructor 1|constructor 2|constructor 3].
       case:ifP; last by move=>_; apply Q2.
       rewrite domPt inE=>/eqP<-; rewrite findPt.
       by case=>????; subst z to' c; rewrite eqxx in N.
-    exists i; split=>[|j[c1]];rewrite findUnL ?(valid_fresh) ?(cohVs (cohQ s C))//.   
-    - by exists c'; rewrite (find_some Q1). 
-    case: ifP=>_; first by move=> T; apply: Q3; exists c1. 
+    exists i; split=>[|j[c1]];rewrite findUnL ?(valid_fresh) ?(cohVs (cohQ s C))//.
+    - by exists c'; rewrite (find_some Q1).
+    case: ifP=>_; first by move=> T; apply: Q3; exists c1.
     by case/findPt_inv=>_[]????; subst to' z; rewrite eqxx in N.
-  by case:G5=>rq[rs][Tr]Np; exists rq, rs; rewrite /getLocal/=findU A/=. 
-    
+  by case:G5=>rq[rs][Tr]Np; exists rq, rs; rewrite /getLocal/=findU A/=.
+
 (* Send-transition, case 2 *)
-- split=>//=; first by rewrite /getLocal/= findU (negbTE N) in G1 *. 
+- split=>//=; first by rewrite /getLocal/= findU (negbTE N) in G1 *.
   + move=>i t c; rewrite findUnR ?(valid_fresh) ?(cohVs (cohQ s C))//.
-    case:ifP; last by move=>_; apply G3. 
+    case:ifP; last by move=>_; apply G3.
     rewrite domPt inE=>/eqP<-; rewrite findPt.
     by case=>????; subst z to'; rewrite eqxx in N.
   + move=>i t c; rewrite findUnR ?(valid_fresh) ?(cohVs (cohQ s C))//.
-    case:ifP; last by move=>_; apply G4. 
+    case:ifP; last by move=>_; apply G4.
     rewrite domPt inE=>/eqP<-; rewrite findPt.
     by case=>????; subst z to'; rewrite eqxx in A.
-  by case:G5=>rq[rs][Tr]Np; exists rq, rs; rewrite /getLocal/=findU A/=. 
+  by case:G5=>rq[rs][Tr]Np; exists rq, rs; rewrite /getLocal/=findU A/=.
 
 (* Send-transition, case 3 *)
-- split=>//=; first by rewrite /getLocal/= findU (negbTE N) in G1 *. 
+- split=>//=; first by rewrite /getLocal/= findU (negbTE N) in G1 *.
   + move=>i t c; rewrite findUnR ?(valid_fresh) ?(cohVs (cohQ s C))//.
-    case:ifP; last by move=>_; apply G3. 
+    case:ifP; last by move=>_; apply G3.
     rewrite domPt inE=>/eqP<-; rewrite findPt.
     by case=>????; subst to' z; rewrite eqxx in N.
   + case: G4; case=>i[[c']Q1 Q3] Q2; split; last first.
@@ -846,31 +837,31 @@ case:M; case=>G1 G2 G3 G4 G5; [constructor 1|constructor 2|constructor 3].
       case:ifP; last by move=>_; apply Q2.
       rewrite domPt inE=>/eqP<-; rewrite findPt.
       by case=>????; subst z to' c; rewrite eqxx in A.
-    exists i; split=>[|j[c1]];rewrite findUnL ?(valid_fresh) ?(cohVs (cohQ s C))//.   
-    - by exists c'; rewrite (find_some Q1). 
-    case: ifP=>_; first by move=> T; apply: Q3; exists c1. 
+    exists i; split=>[|j[c1]];rewrite findUnL ?(valid_fresh) ?(cohVs (cohQ s C))//.
+    - by exists c'; rewrite (find_some Q1).
+    case: ifP=>_; first by move=> T; apply: Q3; exists c1.
     by case/findPt_inv=>_[]????; subst to' z; rewrite eqxx in A.
-  by case:G5=>rq[rs][Tr]Np; exists rq, rs; rewrite /getLocal/=findU A/=. 
+  by case:G5=>rq[rs][Tr]Np; exists rq, rs; rewrite /getLocal/=findU A/=.
 
 (** Receive-transitions **)
 case:M; case=>G1 G2 G3 G4 G5; [constructor 1|constructor 2|constructor 3].
 
 (* Receive-transition, case 1 *)
-- split=>//=; first by rewrite /getLocal/= findU (negbTE N) in G1 *. 
+- split=>//=; first by rewrite /getLocal/= findU (negbTE N) in G1 *.
   + by apply: no_msg_from_to_consume'=>//; rewrite (cohVs (cohQ s C)).
   + case: msg H2 H4=>t c H2 H4.
     apply: (msg_spec_consumeE (cohVs (cohQ s C)) H4 G4).
     by rewrite (negbT A) orbC.
-  by case:G5=>rq[rs][Tr]Np; exists rq, rs; rewrite /getLocal/=findU A/=. 
+  by case:G5=>rq[rs][Tr]Np; exists rq, rs; rewrite /getLocal/=findU A/=.
 
 (* Receive-transition, case 2 *)
-- split=>//=; first by rewrite /getLocal/= findU (negbTE N) in G1 *. 
+- split=>//=; first by rewrite /getLocal/= findU (negbTE N) in G1 *.
   + by apply: no_msg_from_to_consume'=>//; rewrite (cohVs (cohQ s C)).
   + by apply: no_msg_from_to_consume'=>//; rewrite (cohVs (cohQ s C)).
-  by case:G5=>rq[rs][Tr]Np; exists rq, rs; rewrite /getLocal/=findU A/=. 
+  by case:G5=>rq[rs][Tr]Np; exists rq, rs; rewrite /getLocal/=findU A/=.
 
 (* Receive-transition, case 3 *)
-- split=>//=; first by rewrite /getLocal/= findU (negbTE N) in G1 *. 
+- split=>//=; first by rewrite /getLocal/= findU (negbTE N) in G1 *.
   + by apply: no_msg_from_to_consume'=>//; rewrite (cohVs (cohQ s C)).
   + case: msg H2 H4=>t c H2 H4.
     apply: (msg_spec_consumeE (cohVs (cohQ s C)) H4 G4).
@@ -887,7 +878,7 @@ Proof.
 move=>H1 [n]H2; elim: n s H2 H1=>/=[s | n Hi s]; first by case=>Z _; subst s2.
 case=>z[s1][N]H1 H2 H3; apply: (Hi s1 H2).
 by apply: (msg_story_step _ _ _ _ _ _ _ _ N H3 H1).
-Qed.  
+Qed.
 
 
 (**************************************************************)
@@ -899,17 +890,17 @@ Qed.
 Program Definition read_request_id to :
   {rrd : seq (nid * nat) * seq (nid * nat) * Data}, DHT [this, W]
    (fun i =>
-      let: (reqs, resp, data) := rrd in 
+      let: (reqs, resp, data) := rrd in
       [/\ getLq i = qst :-> (reqs, resp),
        local_indicator data (getLc i),
        query_init_state to i &
        core_state_to_data to (getLc' i to) data],
-   fun (r : nat) m => 
-     let: (reqs, resp, data) := rrd in 
+   fun (r : nat) m =>
+     let: (reqs, resp, data) := rrd in
      [/\ getLq m = qst :-> (reqs, resp),
        local_indicator data (getLc m),
        query_init_state to m,
-       core_state_to_data to (getLc' m to) data &                                              
+       core_state_to_data to (getLc' m to) data &
        r = fresh_id reqs]) :=
   Do _ (act (@skip_action_wrapper W this lq pq prEqQ _
                                 (fun s pf => fresh_id (getSt this pf).1))).
@@ -922,10 +913,10 @@ rewrite !(rely_loc' _ R2) !(rely_loc' _ R1); split=>//.
 - apply: (core_state_stable _ _ _ _ R2); [by case: P3|by rewrite !(rely_loc' _ R1)|].
   by apply: (core_state_stable _ _ _ _ R1)=>//; case: P3.
 rewrite -(rely_loc' _ R1) in P1.
-suff X: getSt this (Actions.safe_local prEqQ H1) = (rq, rs) by rewrite X. 
+suff X: getSt this (Actions.safe_local prEqQ H1) = (rq, rs) by rewrite X.
 by move: (getStK (Actions.safe_local prEqQ H1) P1)=>/=.
 Qed.
-    
+
 (********************** Sending request ***********************)
 
 Program Definition send_req rid to :=
@@ -936,14 +927,14 @@ Next Obligation. by rewrite !InE; left. Qed.
 Program Definition send_req_act (rid : nat) (to : nid) :
   {rrd : seq (nid * nat) * seq (nid * nat) * Data}, DHT [this, W]
    (fun i =>
-      let: (reqs, resp, data) := rrd in 
+      let: (reqs, resp, data) := rrd in
       [/\ getLq i = qst :-> (reqs, resp),
        local_indicator data (getLc i),
        rid = fresh_id reqs,
        query_init_state to i &
        core_state_to_data to (getLc' i to) data],
-   fun (r : seq nat) m => 
-     let: (reqs, resp, data) := rrd in 
+   fun (r : seq nat) m =>
+     let: (reqs, resp, data) := rrd in
      [/\ getLq m = qst :-> ((to, rid) :: reqs, resp),
       local_indicator data (getLc m),
       r = [:: rid],
@@ -957,12 +948,12 @@ apply: act_rule=>i1 R0; split=>//=[|r i2 i3[Hs]St R2].
 (* Precondition *)
 - rewrite /Actions.send_act_safe/=.
   move/rely_coh: (R0)=>[_ C1]; rewrite -(rely_loc' _ R0) in P1.
-  move: (coh_coh lq C1); rewrite prEqQ=>Cq1; 
+  move: (coh_coh lq C1); rewrite prEqQ=>Cq1;
   split=>//; [split=>//; try by case:Q| | ].
   + by exists Cq1; rewrite /QueryProtocol.send_req_prec (getStK _ P1)/= P2.
   + by apply/andP; split=>//; rewrite -(cohD C1) W_dom !inE eqxx orbC.
-  move=>z lc hk; rewrite find_umfilt eqxx /query_hookz.
-  move => F.
+  move=>z lc hk; rewrite find_umfiltk eqxx /query_hookz.
+  move=>F.
   apply sym_eq in F.
   move: F.
   by move/find_some; rewrite domPt !inE=>/eqP.
@@ -998,9 +989,9 @@ clear N R2 Q C0 X i3 P3.
 split=>//.
 - rewrite /getStatelet findU; move/negbTE: Lab_neq; rewrite eq_sym=>->//=.
   by rewrite (rely_loc' _ R0).
-constructor 1. 
+constructor 1.
 split=>//; rewrite ?inE ?eqxx=>//=.
-- rewrite locE=>//; 
+- rewrite locE=>//;
   [by rewrite -(cohD C1) W_dom !inE eqxx orbC|
    apply: cohS C1|by apply: cohVl Cq1].
 (* Prove the interesting transition *)
@@ -1008,19 +999,19 @@ split=>//; rewrite ?inE ?eqxx=>//=.
   set ds := (dsoup _); rewrite findUnR; last first.
   by rewrite valid_fresh; apply: cohVs Cq1.
   rewrite domPt !inE/=; case:ifP=>[/eqP<-|_]; last by apply: Q4.
-  by rewrite findPt; case=><-. 
+  by rewrite findPt; case=><-.
 (* TODO: refactor this into a separate lemma about those state predicates *)
 - rewrite /getStatelet findU eqxx (cohS C1)/=.
   set ds := (dsoup _); split=>//.
   exists (fresh ds); split=>//.
   + exists [:: fresh_id reqs].
     rewrite findUnR; last by rewrite valid_fresh; apply: cohVs Cq1.
-    by rewrite domPt inE eqxx findPt. 
+    by rewrite domPt inE eqxx findPt.
   + move=>x[c]; rewrite findUnR; last by rewrite valid_fresh; apply: cohVs Cq1.
-    case:ifP=>[|_[]]; first by rewrite domPt inE=>/eqP->.
+    case:ifP=>[|_]; first by rewrite domPt inE=>/eqP->.
     by move/(Q3 x treq c).
   move=>x c ; rewrite findUnR; last by rewrite valid_fresh; apply: cohVs Cq1.
-  case:ifP=>[|_[]]; last by move/(Q3 x treq c).
+  case:ifP=>[|_]; last by move/(Q3 x treq c).
   by rewrite domPt inE=>/eqP->; rewrite findPt;case=>->.
 set ds := (dsoup _).
 case: Q2=>reqs'[resp'][G1 G2].
@@ -1033,14 +1024,14 @@ case X: (to == this).
        by rewrite -(cohD C1) W_dom !inE eqxx orbC].
 - exists reqs', resp'; split=>//.
   rewrite /getStatelet findU eqxx (cohS C1)/=.
-  by rewrite /getLocal findU X. 
+  by rewrite /getLocal findU X.
 case: (Q)=>Nq _ _ _.
 move: (core_state_stable _ _ _ _ R0 Nq Pi P3)=>H1.
 rewrite -(rely_loc' _ R0) in Pi.
 have Pi': local_indicator d (getLc' i2 this).
-- by rewrite Z'/getStatelet findU/= eq_sym; move/negbTE:Lab_neq->. 
+- by rewrite Z'/getStatelet findU/= eq_sym; move/negbTE:Lab_neq->.
 apply: (core_state_stable _ _ _ _ R2 Nq Pi').
-by rewrite Z'/getStatelet findU/= eq_sym; move/negbTE:Lab_neq->. 
+by rewrite Z'/getStatelet findU/= eq_sym; move/negbTE:Lab_neq->.
 Qed.
 
 (***************** Receiving request in a loop ******************)
@@ -1090,25 +1081,25 @@ Program Definition receive_resp_loop (rid : nat) to :
       local_indicator data (getLc m),
       query_init_state to m,
       core_state_to_data to (getLc' m to) data &
-      d = data]) := 
+      d = data]) :=
   Do _ (@while this W _ _ recv_resp_cond (recv_resp_inv rid to) _
          (fun _ => Do _ (
            r <-- tryrecv_resp rid to;
              match r with
              | Some (from, tg, body) =>
-               ret _ _ (Some (deserialize (behead body)))             
+               ret _ _ (Some (deserialize (behead body)))
              | None => ret _ _ None
-             end              
+             end
          )) None).
 
 Next Obligation. by apply: with_spec x. Defined.
 Next Obligation.
 case: b H=>[b|]; rewrite /recv_resp_inv !(rely_loc' _ H0); case=>H1 H2 H3.
 - move=>H4 ->; split=>//; try by apply: (query_init_rely _ _ _ H3 H0).
-- by apply: (core_state_stable _ _ _ _ H0 _ H2)=>//; case: H3. 
+- by apply: (core_state_stable _ _ _ _ H0 _ H2)=>//; case: H3.
 split=>//; try apply: (msg_story_rely _ _ _ _ _ _ _ H3 H0).
 Defined.
-  
+
 Next Obligation.
 rename H into d.
 apply: ghC=>i0 [[reqs resp] data][G0 H0] C0; apply: step.
@@ -1121,12 +1112,12 @@ case=>[[[from tg] body] i2 i3|i2 i3]; last first.
   by apply: (msg_story_rely _ _ _ _ _ _ _ _ R4);
     apply: (msg_story_rely _ _ _ _ _ _ _ _ R3);
     apply: (msg_story_rely _ _ _ _ _ _ _ _ R1).
-case=>Sf[]C1[]=>[|[l'][mid][tms][from'][rt][pf][][E]Hin E2 Hw/=]; first by case. 
+case=>Sf[]C1[]=>[|[l'][mid][tms][from'][rt][pf][][E]Hin E2 Hw/=]; first by case.
 case/andP=>/eqP Z1/andP[/eqP Z2]/andP[/eqP Z3]/andP[/eqP Z4]Qn->{i2}[Z5] Z6 Z7 R3.
 subst l' from' from tg body rid.
 move: rt pf (coh_s (w:=W) lq (s:=i1) C1) Hin R3 E2 Hw Z3 E; rewrite !prEqQ.
 move=>/=rt pf C1' Hin R E2 Hw G E.
-have D: rt = qrecv_resp _ by move: Hin G; do![case=>/=; first by move=>->].  
+have D: rt = qrecv_resp _ by move: Hin G; do![case=>/=; first by move=>->].
 subst rt=>{G}; simpl in E2.
 set i2 := (upd _ _ _) in R.
 apply: ret_rule=>i4 R3/=; rewrite !(rely_loc' _ R3)!(rely_loc' _ R).
@@ -1138,26 +1129,26 @@ suff X : [/\ getLocal this (getStatelet i2 lq) = qst :-> (reqs, resp),
   by apply: (query_init_rely _ _ _ _ R3); apply: (query_init_rely _ _ _ _ R).
 - case: d G0 H0=>//=_[_ H2][_] H3 _ _; case: X3=>Nq _ _ _.
   move: (X2); rewrite -(rely_loc' _ R)=>X3.
-  apply: (core_state_stable _ _ _ _ R3 Nq X3).  
-  apply: (core_state_stable _ _ _ _ R Nq X2).  
+  apply: (core_state_stable _ _ _ _ R3 Nq X3).
+  apply: (core_state_stable _ _ _ _ R Nq X2).
   move: (core_state_stable _ _ _ _ R1 Nq H2 H3)=>{H2 H3 X3 X4}Y.
-  by subst i2; rewrite /getStatelet findU eq_sym; move/negbTE:Lab_neq=>->.  
-clear R i4 R3.  
+  by subst i2; rewrite /getStatelet findU eq_sym; move/negbTE:Lab_neq=>->.
+clear R i4 R3.
 case: d G0 H0=>//=_[Q1 Q2 Q3]; rewrite -!(rely_loc' _ R1) in Q1 Q2.
 move: (msg_story_rely _ _ _ _ _ _ _ Q3 R1)=>{Q3}Q3.
 have P1: valid (dstate (getSq i1)) by case: (C1')=>P1 P2 P3 P4.
 have P2: valid i1 by apply: (cohS C1).
 have P3: lq \in dom i1.
-  rewrite -(cohD C1) domUn inE !domPt !inE/= inE eqxx orbC andbC/=.
+  rewrite -(cohD C1) domUn inE !domPt !inE /= eqxx orbC andbC/=.
   by case/andP: W_valid.
-clear Hin R1 C0 i0 i3 Hw. 
+clear Hin R1 C0 i0 i3 Hw.
 (* Consider different cases for msg_story. *)
 case: Q3=>_ Q3 Q4 [].
 (* Now dismiss two first disjuncts. *)
 - case=>_/(_ mid (tag tms) (tms_cont tms)); rewrite -E.
-  by case: (tms)E2=>t c/=E2=>/(_ (erefl _))/=; subst t. 
+  by case: (tms)E2=>t c/=E2=>/(_ (erefl _))/=; subst t.
 - case=>_ _ _/(_ mid (tag tms) (tms_cont tms)); rewrite -E.
-  by case: (tms)E2=>t c/=E2=>/(_ (erefl _))/=; subst t. 
+  by case: (tms)E2=>t c/=E2=>/(_ (erefl _))/=; subst t.
 (* The interesting part *)
 case=>X1 _ X2 X3 X4; rewrite /query_init_state.
 subst i2.
@@ -1173,7 +1164,7 @@ split=>//; last 1 first.
   by move/(_ _ _ E)=>/eqP->/=; apply: ds_inverse.
 - by rewrite /getStatelet findU eq_sym; move/negbTE:Lab_neq=>->.
 split=>//.
-- case B: (to == this); last first. 
+- case B: (to == this); last first.
   + rewrite /getStatelet findU eqxx/= (cohS C1)/=.
     rewrite /holds_res_perms in X4.
     case: X4=> rq[rs][G1 G2]; exists rq, rs; split=>//.
@@ -1182,8 +1173,8 @@ split=>//.
   rewrite G1 in X1.
   have V: valid (qst :-> (rq, rs)) by apply: validPt.
   case: (hcancelPtV V X1)=>Z1 Z2; subst rq rs; exists reqs, resp; split=>//.
-  rewrite /getStatelet/= findU eqxx (cohS C1)/=/getLocal/=findU eqxx/=. 
-  by case: C1'=>_->. 
+  rewrite /getStatelet/= findU eqxx (cohS C1)/=/getLocal/=findU eqxx/=.
+  by case: C1'=>_->.
 - rewrite /getStatelet/= findU eqxx/= (cohS C1)/=.
   by apply: (no_msg_from_to_consume' _ X2); case: C1'; case.
 rewrite /getStatelet/= findU eqxx/= (cohS C1)/=.
@@ -1206,7 +1197,7 @@ Variable default_data : Data.
 Program Definition request_data_program to :
   {rrd : seq (nid * nat) * seq (nid * nat) * Data}, DHT [this, W]
    (fun i =>
-      let: (reqs, resp, data) := rrd in 
+      let: (reqs, resp, data) := rrd in
       [/\ getLq i = qst :-> (reqs, resp),
        local_indicator data (getLc i),
        query_init_state to i &
@@ -1222,7 +1213,7 @@ Program Definition request_data_program to :
      rid <-- read_request_id to;
      send_req_act rid to;;
      r <-- receive_resp_loop rid to;
-     ret _ _ (if r is Some d then d else default_data) 
+     ret _ _ (if r is Some d then d else default_data)
      ).
 Next Obligation.
 apply:ghC=>i1[[reqs resp] d][L1 I1 M1 S1] C1.
@@ -1234,7 +1225,7 @@ apply: step; apply: (gh_ex (g:=(reqs, resp, d))).
 apply: call_rule=>//? i4[d'][->][T1] T2 T3 T4->{d'}C4.
 apply: ret_rule=>i5 R; rewrite !(rely_loc' _ R); split=>//.
 - by apply: (query_init_rely _ _ _ _ R).
-by apply: (core_state_stable _ _ _ _ R _ T2 T4); case: T3.  
+by apply: (core_state_stable _ _ _ _ R _ T2 T4); case: T3.
 Qed.
 
 End QueryHooked.
