Examples/TwoPhaseCommit/TwoPhaseCoordinator.v
@@ -80,13 +80,13 @@ Export TPCProtocol.
 
 Program Definition read_round :
   {(ecl : (nat * CState) * Log)}, DHT [cn, W]
-  (fun i => loc i = st :-> ecl.1 \+ log :-> ecl.2, 
+  (fun i => loc i = st :-> ecl.1 \+ log :-> ecl.2,
    fun r m => loc m = st :-> ecl.1 \+ log :-> ecl.2 /\
               exists (pf : coh (getS m)), r = (getStC pf).1) :=
   Do (act (@skip_action_wrapper W cn l tpc (prEq tpc) _
                                 (fun s pf => (getStC pf).1))).
 Next Obligation.
-apply: ghC=>i [[e c]lg]/= E _. 
+apply: ghC=>i [[e c]lg]/= E _.
 apply: act_rule=>j R; split=>[|r k m]; first by case: (rely_coh R).
 case=>/=H1[Cj]Z; subst j=>->R'.
 split; first by rewrite (rely_loc' l R') (rely_loc' _ R).
@@ -103,29 +103,29 @@ Qed.
 (*******************************************)
 
 Definition send_prep_loop_spec (e : nat) d := forall to_send,
-  {l : Log}, DHT [cn, W] 
+  {l : Log}, DHT [cn, W]
   (fun i =>
      loc i = st :-> (e, CInit) \+ log :-> l /\ perm_eq pts to_send \/
      if to_send == [::]
-     then loc i = st :-> (e, CWaitPrepResponse d [::]) \+ log :-> l 
+     then loc i = st :-> (e, CWaitPrepResponse d [::]) \+ log :-> l
      else exists (ps : seq nid),
          loc i = st :-> (e, CSentPrep d ps) \+ log :-> l /\
          perm_eq pts (ps ++ to_send),
    fun r m => r = tt /\ loc m = st :-> (e, CWaitPrepResponse d [::]) \+ log :-> l).
 
 Program Definition send_prep_loop e d :
-  {l : Log}, DHT [cn, W] 
+  {l : Log}, DHT [cn, W]
   (fun i => loc i = st :-> (e, CInit) \+ log :-> l,
    fun r m => r = tt /\
               loc m = st :-> (e, CWaitPrepResponse d [::]) \+ log :-> l) :=
-  Do (ffix (fun (rec : send_prep_loop_spec e d) to_send => 
+  Do (ffix (fun (rec : send_prep_loop_spec e d) to_send =>
               Do (match to_send with
                   | to :: tos => send_prep e d to ;; rec tos
                   | [::] => ret _ _ tt
                   end)) pts).
 
 (* Verifying the loop invariant *)
-Next Obligation. 
+Next Obligation.
 apply: ghC=>i1 lg.
 (*********************************)
 (* two cases of the precondition *)
@@ -137,8 +137,8 @@ case=>[[E1 P1 C1]|].
 (*--------------------------------------*)
 
 - case: to_send P1=>[|to tos Hp].
-  + by move/perm_size=>/=/size0nil=>Z; rewrite Z in (PtsNonEmpty). 
-- apply: step; apply:act_rule=>j1 R1/=; split=>[|r k m[Sf]St R2]. 
+  + by move/perm_size=>/=/size0nil=>Z; rewrite Z in (PtsNonEmpty).
+- apply: step; apply:act_rule=>j1 R1/=; split=>[|r k m[Sf]St R2].
   split=>//=; first by case: (rely_coh R1).
   + split; first by split=>//; move/perm_mem: Hp->; rewrite inE eqxx.
     case: (proj2 (rely_coh R1))=>_ _ _ _/(_ l); rewrite (prEq tpc)=>C; exists C.
@@ -167,13 +167,13 @@ have Pre:
 - case X: ([::] == tos);[move/eqP: X=>X; subst tos; rewrite eqxx|
                          rewrite eq_sym X].
   have Y: pts == [:: to] by rewrite (perm_small_eq _ Hp).
-  rewrite /cstep_send/= Y in G. 
+  rewrite /cstep_send/= Y in G.
   move: (proj2 Hc)=>Y'; rewrite Y' in G=>{Y'}.
   rewrite [cn_safe_coh _ ](pf_irr _ C) E1' in G. (* TADA! *)
   rewrite (rely_loc' l R2); subst k; rewrite -(rely_loc' _ R1) in E1.
   rewrite locE; last apply: (cohVl C).
   + by rewrite -(pf_irr (cn_in cn pts others) (cn_this_in _ _))
-                  (getStL_Kc _ (cn_in cn pts others) E1). 
+                  (getStL_Kc _ (cn_in cn pts others) E1).
   + by rewrite -(cohD (proj2 (rely_coh R1)))/ddom domPt inE/=.
   by apply: (cohS (proj2 (rely_coh R1))).
 - exists [:: to]; split; last by rewrite cat_cons/=.
@@ -185,18 +185,18 @@ have Pre:
     move: F.
     by case=>/size0nil=>Z'; rewrite Z' eqxx in X.
     (* This part is similar to the previous step *)
-  rewrite /cstep_send/= Y in G. 
+  rewrite /cstep_send/= Y in G.
   move: (proj2 Hc)=>Y'; rewrite Y' in G=>{Y'}.
   rewrite [cn_safe_coh _ ](pf_irr _ C) E1' in G. (* TADA! *)
   rewrite (rely_loc' l R2); subst k; rewrite -(rely_loc' _ R1) in E1.
   rewrite locE; last apply: (cohVl C).
   + by rewrite -(pf_irr (cn_in cn pts others) (cn_this_in _ _))
-                  (getStL_Kc _ (cn_in cn pts others) E1). 
+                  (getStL_Kc _ (cn_in cn pts others) E1).
   + by rewrite -(cohD (proj2 (rely_coh R1)))/ddom domPt inE/=.
   by apply: (cohS (proj2 (rely_coh R1))).
 
 apply: call_rule'=>/=[Cm|r2 m2]; first by right.
-by case=>//; right. 
+by case=>//; right.
 
 (*------------------------------------------*)
 (* Case 2: We are in the intermediate state *)
@@ -213,7 +213,7 @@ have Y: exists to tos, to_send = to :: tos.
 - case: to_send X Hp; first by rewrite eqxx.
   by move=>to tos _ _; exists to, tos.
 case: Y=>to[tos] Z; subst to_send=>{X}.
-- apply: step; apply:act_rule=>j1 R1/=; split=>[|r k m[Sf]St R2]. 
+- apply: step; apply:act_rule=>j1 R1/=; split=>[|r k m[Sf]St R2].
   split=>//=; first by case: (rely_coh R1).
   + split; first by split=>//; move/perm_mem: Hp->;
                     rewrite mem_cat orbC inE eqxx.
@@ -233,12 +233,12 @@ case: Y=>to[tos] Z; subst to_send=>{X}.
   apply sym_eq in F.
   move: F.
   by move/find_some; rewrite dom0.
-(* dismiss the bogus branch *)    
-case: {-1}(Sf)=>_/=[]Hc[C][]. 
+(* dismiss the bogus branch *)
+case: {-1}(Sf)=>_/=[]Hc[C][].
 - case=>b[E1'][d'][Z1 Z2]_; subst b d'.
   rewrite -(rely_loc' _ R1) in E1.
   by rewrite (getStC_K C E1) in E1'; discriminate E1'.
-move=>[n][d'][ps'][E1'][]Z1 Z2 N _ _; subst n d'. 
+move=>[n][d'][ps'][E1'][]Z1 Z2 N _ _; subst n d'.
 rewrite -(rely_loc' _ R1) in E1.
 move: (E1'); rewrite (getStC_K C E1); case=>Z; subst ps'.
 move: St=>[Z][h][[]Z' G]; subst r h.
@@ -258,13 +258,13 @@ suff Pre:
     rewrite [cn_safe_coh _ ](pf_irr _ C) E1' in G.
   have Y: perm_eq (to :: ps) pts.
     rewrite (perm_sym pts) in Hp.
-    by apply/permEl; rewrite -cat1s perm_catC; apply/permPl. 
-  rewrite Y/= in G.     
+    by apply/permEl; rewrite -cat1s perm_catC; apply/permPl.
+  rewrite Y/= in G.
   rewrite (rely_loc' l R2); subst k; rewrite locE; last apply: (cohVl C).
   + by rewrite -(pf_irr (cn_in cn pts others) (cn_this_in _ _))
-               (getStL_Kc _ (cn_in cn pts others) E1). 
+               (getStL_Kc _ (cn_in cn pts others) E1).
   + by rewrite -(cohD (proj2 (rely_coh R1)))/ddom domPt inE/=.
-  by apply: (cohS (proj2 (rely_coh R1))).   
+  by apply: (cohS (proj2 (rely_coh R1))).
 
 rewrite /cstep_send/= (proj2 Hc)/= in G.
 rewrite [cn_safe_coh _ ](pf_irr _ C) E1' in G.
@@ -278,14 +278,14 @@ have Y : perm_eq (to :: ps) pts = false.
   apply sym_eq in F.
   move: F.
   by move/size0nil=>Z; subst tos.
-rewrite Y/= in G.     
+rewrite Y/= in G.
 rewrite (rely_loc' l R2); subst k; rewrite locE; last apply: (cohVl C).
   + rewrite -(pf_irr (cn_in cn pts others) (cn_this_in _ _))
                (getStL_Kc _ (cn_in cn pts others) E1); exists (to::ps).
     split=>//; move: Hp.
-    by rewrite -cat_rcons -cat1s -!catA !(perm_sym pts) -perm_catCA catA cats1. 
+    by rewrite -cat_rcons -cat1s -!catA !(perm_sym pts) -perm_catCA catA cats1.
   + by rewrite -(cohD (proj2 (rely_coh R1)))/ddom domPt inE/=.
-  by apply: (cohS (proj2 (rely_coh R1))).   
+  by apply: (cohS (proj2 (rely_coh R1))).
 Qed.
 
 (* Verifying the top-level call of ffix *)
@@ -309,7 +309,7 @@ Definition rc_prep_inv (e : nat) (dl : data * Log) : cont (seq (nid * bool)) :=
 Program Definition receive_prep_loop (e : nat):
   {(dl : data * Log)}, DHT [cn, W]
   (fun i => loc i = st :-> (e, CWaitPrepResponse dl.1 [::]) \+ log :-> dl.2,
-   fun res m => 
+   fun res m =>
        loc m = st :-> (e, CWaitPrepResponse dl.1 res) \+ log :-> dl.2 /\
        (perm_eq (map fst res) pts))
   :=
@@ -322,7 +322,7 @@ Program Definition receive_prep_loop (e : nat):
                then ret _ _ ((from, tg == prep_yes) :: acc)
                else ret _ _ acc
            | None => ret _ _ acc
-           end              
+           end
         )) [::]).
 
 (* TODO: Get rid of this bogus obligation! *)
@@ -334,20 +334,20 @@ move=>i[[d lg]]/=[H1 I1]; apply: step.
 apply: act_rule=>j R1/=; split; first by case: (rely_coh R1).
 case=>[[[from tg] body] k m|k m]; last first.
 - case=>Sf []Cj[]H; last by case: H=>[?][?][?][?][?][?][].
-  have E: k = j by case: H. 
+  have E: k = j by case: H.
   move: H; subst k=>_ R2; apply: ret_rule=>m' R3 {d lg I1}[d lg][H2].
   by rewrite /rc_prep_inv; rewrite -(rely_loc' _ R1)-(rely_loc' _ R2)-(rely_loc' _ R3).
 case=>Sf []Cj[]=>[|[l'][mid][tms][from'][rt][pf][][E]Hin E1 Hw/=]; first by case.
 case/andP=>/eqP Z G->{k}[]Z1 Z2 Z3 R2; subst l' from' tg body.
-move: rt pf (coh_s (w:=W) l (s:=j) Cj) Hin R2 E1 Hw G E; rewrite prEq/=. 
+move: rt pf (coh_s (w:=W) l (s:=j) Cj) Hin R2 E1 Hw G E; rewrite prEq/=.
 move=>rt pf Cj' Hin R E1 Hw G E.
 have D: rt = cn_receive_prep_yes_trans _ _ _ \/ rt = cn_receive_prep_no_trans _ _ _.
 - case: Hin G=>/=; first by intuition.
   case; first by intuition.
-  by do! [case; first by move=>->]. 
+  by do! [case; first by move=>->].
 (* Some forward facts: *)
 have P1: valid (dstate (getS j))
-  by apply: (@cohVl _ TPCCoh); case: (Cj')=>P1 P2 P3 P4; split=>//=; done. 
+  by apply: (@cohVl _ TPCCoh); case: (Cj')=>P1 P2 P3 P4; split=>//=; done.
 have P2: valid j by apply: (cohS (proj2 (rely_coh R1))).
 have P3: l \in dom j by rewrite -(cohD (proj2 (rely_coh R1)))/ddom domPt inE/=.
 (* Two cases: received yes or no from a participant *)
@@ -380,11 +380,11 @@ Program Definition read_resp_result :
   {(e : nat) (d : data) (lg : Log) res}, DHT [cn, W]
   (fun i => loc i = st :-> (e, CWaitPrepResponse d res) \+ log :-> lg,
    fun r m => loc m = st :-> (e, CWaitPrepResponse d res) \+ log :-> lg /\
-              r = all (fun i => i) (map snd res)) :=                        
+              r = all (fun i => i) (map snd res)) :=
   Do (act (@skip_action_wrapper W cn l tpc (prEq tpc) _
           (fun s pf => all (fun i => i) (map snd (read_res (getStC pf)))))).
 Next Obligation.
-move=>/=i[e][d][lg][res] E/=. 
+move=>/=i[e][d][lg][res] E/=.
 apply: act_rule=>j R; split=>/=[|r k m]; first by case: (rely_coh R).
 case=>/=H1[Cj]Z; subst j=>->R'.
 split; first by rewrite (rely_loc' l R') (rely_loc' _ R).
@@ -396,7 +396,7 @@ Qed.
 (*************************)
 
 Program Definition coordinator_prelude (d : data) :
-  {(lg : Log)}, DHT [cn, W] 
+  {(lg : Log)}, DHT [cn, W]
   (fun i => exists (e : nat), loc i = st :-> (e, CInit) \+ log :-> lg,
    fun r m => let: (res, b) := r in
        exists (e : nat),
@@ -405,7 +405,7 @@ Program Definition coordinator_prelude (d : data) :
            b = all id (map snd res)]) :=
   Do (e <-- read_round;
       send_prep_loop e d;;
-      res <-- receive_prep_loop e;                     
+      res <-- receive_prep_loop e;
       b <-- read_resp_result;
       ret _ _ (res, b)).
 Next Obligation.
@@ -422,9 +422,9 @@ apply: step; apply: (gh_ex (g:=e)); apply: (gh_ex (g:=d));
 apply: call_rule=>// b s4 [E4]->{b}C4/=.
 apply: ret_rule=>i5 R5 lg'[e'] E0'; exists e.
 rewrite E0 in E0'; case: (hcancelV _ E0'); first by rewrite validPtUn.
-case=>Z1 _; subst e'; move/(hcancelPtV _)=>/=.
+case=>Z1 _; subst e'; move/(hcancelPtV _).
 by rewrite validPt (rely_loc' _ R5)=>/(_ is_true_true)=><-.
-Qed.                                                     
+Qed.
 
 (*******************************************)
 (***    Sending commits/aborts           ***)
@@ -456,7 +456,7 @@ Program Definition send_commit_loop e d : send_commit_loop_spec e d :=
 
 Next Obligation.
 apply: ghC=>s1 lg E1 C1; elim: to_send s1 E1 C1=>//=.
-- move=>s1; case; first by case=>?[]_ Z; rewrite -Z in (PtsNonEmpty). 
+- move=>s1; case; first by case=>?[]_ Z; rewrite -Z in (PtsNonEmpty).
   by move=>E1 _; apply: ret_rule=>i2 R; rewrite (rely_loc' _ R).
 move=>to tos Hi s1 H C1.
 apply: step; apply: act_rule=>s2 R2/=.
@@ -473,7 +473,7 @@ have Pre: Actions.send_act_safe W (p:=tpc) cn l
   case: (proj2 (rely_coh R2))=>_ _ _ _/(_ l); rewrite prEq=>C; split.
   + split=>//; case: H; first by case=>?[_]<-; rewrite inE eqxx.
     by case=>ps[_]/perm_mem->; rewrite mem_cat orbC inE eqxx.
-  exists C; case:H=>[[res][P1]P2 P3|[ps][P1 P2]];[left|right];  
+  exists C; case:H=>[[res][P1]P2 P3|[ps][P1 P2]];[left|right];
   rewrite -(rely_loc' _ R2) in P1; rewrite (getStC_K _ P1);
   first by exists e, d, res=>//.
   exists e, d, ps; split=>//.
@@ -482,33 +482,33 @@ have Pre: Actions.send_act_safe W (p:=tpc) cn l
   apply sym_eq in F.
   move: F.
   rewrite -cat_rcons cat_uniq -cats1 cat_uniq=>/andP[]/andP[_]/andP[].
-  by rewrite /= orbC.                                                          
-  
-(* Using the postcondition *)  
+  by rewrite /= orbC.
+
+(* Using the postcondition *)
 split=>// body i3 i4[Sf]/=St R3.
-apply: Hi; last by case: (rely_coh R3).  
+apply: Hi; last by case: (rely_coh R3).
 right; rewrite (rely_loc' _ R3).
-case: (Sf)=>C2/=[][]_ Tp [C2']/=; case; move=>[e'][d']. 
-- move=>[res][E'][]Z P1 P2/andP[P3] _; subst e'. 
+case: (Sf)=>C2/=[][]_ Tp [C2']/=; case; move=>[e'][d'].
+- move=>[res][E'][]Z P1 P2/andP[P3] _; subst e'.
   case: H=>[[res'][E1]Te _ _|[ps]]; last first.
   + by rewrite -(rely_loc' _ R2)=>[][E1]; rewrite (getStC_K _ E1) in E'.
   rewrite -(rely_loc' _ R2) in E1; rewrite (getStC_K _ E1) in E'.
   case: E'=>Z Z'; subst res' d'.
   case: St=>Z1[h][];case=>->{h}; subst body=>G.
-  rewrite (getStC_K _ E1) (getStL_Kc _ _ E1) 
+  rewrite (getStC_K _ E1) (getStL_Kc _ _ E1)
           /cstep_send -{1}Te inE eqxx/= P1 P2 in G.
   have X: (pts == [:: to]) = (tos == [::]).
   + rewrite -Te; apply/Bool.eq_iff_eq_true.
     by split; [move=>/eqP[]->|move/eqP->;rewrite eqxx].
     rewrite X in G; subst i3.
     rewrite locE//; [|by apply: (cohS C2)|by apply: (cohVl C2')].
-  by case: ifP=>X'; rewrite X'//; exists [::to]; split=>//; rewrite -Te. 
-case=>ps[E'][]Z N/andP[P1]_; subst e'.   
+  by case: ifP=>X'; rewrite X'//; exists [::to]; split=>//; rewrite -Te.
+case=>ps[E'][]Z N/andP[P1]_; subst e'.
 case: H=>[[res'][E1]Te _ _|[ps']].
 - by rewrite -(rely_loc' _ R2) in E1; rewrite (getStC_K _ E1) in E'.
 rewrite -(rely_loc' _ R2)=>[][E1] P2; rewrite (getStC_K _ E1) in E'.
 case: E'=>Z1 Z2; subst d' ps'; case: St=>Z1[h][];case=>->{h}; subst body=>G.
-rewrite (getStC_K _ E1) (getStL_Kc _ _ E1) 
+rewrite (getStC_K _ E1) (getStL_Kc _ _ E1)
         /cstep_send Tp in G.
 have X: perm_eq (to :: ps) pts = (tos == [::]).
 - apply/Bool.eq_iff_eq_true; split.
@@ -520,7 +520,7 @@ have X: perm_eq (to :: ps) pts = (tos == [::]).
     move => F.
     apply sym_eq in F.
     move: F.
-    by move/size0nil=>Z; subst tos. 
+    by move/size0nil=>Z; subst tos.
   move/eqP=>Z; subst tos; rewrite perm_sym; apply: (perm_trans P2).
   by apply/permEl; move: (perm_catC ps [:: to]).
 rewrite X in G=>{X}; subst i3.
@@ -540,7 +540,7 @@ Program Definition send_commits e d :
   := Do (send_commit_loop e d pts).
 Next Obligation.
 apply: ghC=>i lg[res][H1]H2 H3 C; apply: (gh_ex (g:=lg)).
-apply: call_rule=>//; first by move=>_; left; exists res. 
+apply: call_rule=>//; first by move=>_; left; exists res.
 Qed.
 
 (* Abort *)
@@ -569,7 +569,7 @@ Program Definition send_abort_loop e d : send_abort_loop_spec e d :=
 
 Next Obligation.
 apply: ghC=>s1 lg E1 C1; elim: to_send s1 E1 C1=>//=.
-- move=>s1; case; first by case=>?[]_ Z; rewrite -Z in (PtsNonEmpty). 
+- move=>s1; case; first by case=>?[]_ Z; rewrite -Z in (PtsNonEmpty).
   by move=>E1 _; apply: ret_rule=>i2 R; rewrite (rely_loc' _ R).
 move=>to tos Hi s1 H C1.
 apply: step; apply: act_rule=>s2 R2/=.
@@ -595,14 +595,14 @@ have Pre: Actions.send_act_safe W (p:=tpc) cn l
   apply sym_eq in F.
   move: F.
   rewrite -cat_rcons cat_uniq -cats1 cat_uniq=>/andP[]/andP[_]/andP[].
-  by rewrite /= orbC.                                                          
+  by rewrite /= orbC.
 
-(* Using the postcondition *)  
+(* Using the postcondition *)
 split=>// body i3 i4[Sf]/=St R3.
-apply: Hi; last by case: (rely_coh R3).  
+apply: Hi; last by case: (rely_coh R3).
 right; rewrite (rely_loc' _ R3).
-case: (Sf)=>C2/=[][]_ Tp [C2']/=; case; move=>[e'][d']. 
-- move=>[res][E'][]Z P1 P2/andP[P3] _; subst e'. 
+case: (Sf)=>C2/=[][]_ Tp [C2']/=; case; move=>[e'][d'].
+- move=>[res][E'][]Z P1 P2/andP[P3] _; subst e'.
   case: H=>[[res'][E1]Te _ _|[ps]]; last first.
   + by rewrite -(rely_loc' _ R2)=>[][E1]; rewrite (getStC_K _ E1) in E'.
   rewrite -(rely_loc' _ R2) in E1; rewrite (getStC_K _ E1) in E'.
@@ -610,20 +610,20 @@ case: (Sf)=>C2/=[][]_ Tp [C2']/=; case; move=>[e'][d'].
   case: St=>Z1[h][];case=>->{h}; subst body=>G.
   have P2' : all id [seq i.2 | i <- res] = false
     by rewrite has_predC in P2; apply/negbTE.
-  rewrite (getStC_K _ E1) (getStL_Kc _ _ E1) 
+  rewrite (getStC_K _ E1) (getStL_Kc _ _ E1)
           /cstep_send -{1}Te inE eqxx/= P1 P2' in G.
   have X: (pts == [:: to]) = (tos == [::]).
   + rewrite -Te; apply/Bool.eq_iff_eq_true.
     by split; [move=>/eqP[]->|move/eqP->;rewrite eqxx].
     rewrite X in G; subst i3.
     rewrite locE//; [|by apply: (cohS C2)|by apply: (cohVl C2')].
-  by case: ifP=>X'; rewrite X'//; exists [::to]; split=>//; rewrite -Te. 
-case=>ps[E'][]Z N/andP[P1]_; subst e'.   
+  by case: ifP=>X'; rewrite X'//; exists [::to]; split=>//; rewrite -Te.
+case=>ps[E'][]Z N/andP[P1]_; subst e'.
 case: H=>[[res'][E1]Te _ _|[ps']].
 - by rewrite -(rely_loc' _ R2) in E1; rewrite (getStC_K _ E1) in E'.
 rewrite -(rely_loc' _ R2)=>[][E1] P2; rewrite (getStC_K _ E1) in E'.
 case: E'=>Z1 Z2; subst d' ps'; case: St=>Z1[h][];case=>->{h}; subst body=>G.
-rewrite (getStC_K _ E1) (getStL_Kc _ _ E1) 
+rewrite (getStC_K _ E1) (getStL_Kc _ _ E1)
         /cstep_send Tp in G.
 have X: perm_eq (to :: ps) pts = (tos == [::]).
 - apply/Bool.eq_iff_eq_true; split.
@@ -635,7 +635,7 @@ have X: perm_eq (to :: ps) pts = (tos == [::]).
     move => F.
     apply sym_eq in F.
     move: F.
-    by move/size0nil=>Z; subst tos. 
+    by move/size0nil=>Z; subst tos.
   move/eqP=>Z; subst tos; rewrite perm_sym; apply: (perm_trans P2).
   by apply/permEl; move: (perm_catC ps [:: to]).
 rewrite X in G=>{X}; subst i3.
@@ -655,7 +655,7 @@ Program Definition send_aborts e d :
   := Do (send_abort_loop e d pts).
 Next Obligation.
 apply: ghC=>i lg[res][H1]H2 H3 C; apply: (gh_ex (g:=lg)).
-apply: call_rule=>//; first by move=>_; left; exists res. 
+apply: call_rule=>//; first by move=>_; left; exists res.
 Qed.
 
 
@@ -678,7 +678,7 @@ Definition rc_commit_inv (e : nat) (dl : data * Log) : cont (seq nid) :=
 Program Definition receive_commit_loop (e : nat):
   {(dl : data * Log)}, DHT [cn, W]
   (fun i => loc i = st :-> (e, CWaitAckCommit dl.1 [::]) \+ log :-> dl.2,
-   fun (res : seq nat) m => 
+   fun (res : seq nat) m =>
        loc m = st :-> (e.+1, CInit) \+ log :-> rcons dl.2 (true, dl.1))
   :=
   Do _ (@while cn W _ _ rc_commit_cond (rc_commit_inv e) _
@@ -690,7 +690,7 @@ Program Definition receive_commit_loop (e : nat):
                then ret _ _ (from :: acc)
                else ret _ _ acc
            | None => ret _ _ acc
-           end              
+           end
         )) [::]).
 
 Next Obligation. by apply: with_spec x. Defined.
@@ -725,7 +725,7 @@ rewrite /rc_step eqxx/cstep_recv/=;
 move/negbTE: I1=>I1; rewrite I1 in Ej *;
 rewrite (getStC_K Cj' Ej) (getStL_Kc _ _ Ej) ?eqxx/=;
 move: G1; case: (from \in pts)=>//=;case: (head 0 tms == e)=>//=;
-case: (from \in acc)=>//=_; case:ifP=>X; rewrite X//=. 
+case: (from \in acc)=>//=_; case:ifP=>X; rewrite X//=.
 Qed.
 
 Next Obligation.
@@ -733,7 +733,7 @@ apply: ghC=>i[d lg]E1 C1.
 have Pre: rc_commit_inv e (d, lg) [::] i.
 - rewrite /rc_commit_inv/= E1/=.
   have X: perm_eq [::] pts = false.
-  - apply/negP. 
+  - apply/negP.
     move/perm_size.
     move => F.
     apply sym_eq in F.
@@ -761,7 +761,7 @@ Definition rc_abort_inv (e : nat) (dl : data * Log) : cont (seq nid) :=
 Program Definition receive_abort_loop (e : nat):
   {(dl : data * Log)}, DHT [cn, W]
   (fun i => loc i = st :-> (e, CWaitAckAbort dl.1 [::]) \+ log :-> dl.2,
-   fun (res : seq nat) m => 
+   fun (res : seq nat) m =>
        loc m = st :-> (e.+1, CInit) \+ log :-> rcons dl.2 (false, dl.1))
   :=
   Do _ (@while cn W _ _ rc_abort_cond (rc_abort_inv e) _
@@ -773,7 +773,7 @@ Program Definition receive_abort_loop (e : nat):
                then ret _ _ (from :: acc)
                else ret _ _ acc
            | None => ret _ _ acc
-           end              
+           end
         )) [::]).
 
 Next Obligation. by apply: with_spec x. Defined.
@@ -808,7 +808,7 @@ rewrite /rc_step eqxx/cstep_recv/=;
 move/negbTE: I1=>I1; rewrite I1 in Ej *;
 rewrite (getStC_K Cj' Ej) (getStL_Kc _ _ Ej) ?eqxx/=;
 move: G1; case: (from \in pts)=>//=;case: (head 0 tms == e)=>//=;
-case: (from \in acc)=>//=_; case:ifP=>X; rewrite X//=. 
+case: (from \in acc)=>//=_; case:ifP=>X; rewrite X//=.
 Qed.
 
 Next Obligation.
@@ -816,7 +816,7 @@ apply: ghC=>i[d lg]E1 C1.
 have Pre: rc_abort_inv e (d, lg) [::] i.
 - rewrite /rc_abort_inv/= E1/=.
   have X: perm_eq [::] pts = false.
-  - apply/negP. 
+  - apply/negP.
     move/perm_size.
     move => F.
     apply sym_eq in F.
@@ -828,25 +828,25 @@ apply: call_rule'=>[|acc m]; first by exists (d, lg).
 case/(_ (d, lg) Pre)=>/=H1 H2 Cm.
 by move/negbNE: H1=>H1; rewrite /rc_abort_inv H1 in H2.
 Qed.
- 
+
 (*****************************************************)
 (*      Full coordinator Implementation              *)
 (*****************************************************)
 
 Program Definition coordinator_round (d : data) :
-  {(e : nat)(lg : Log)}, DHT [cn, W] 
+  {(e : nat)(lg : Log)}, DHT [cn, W]
   (fun i => loc i = st :-> (e, CInit) \+ log :-> lg,
    fun res m => loc m = st :-> (e.+1, CInit) \+ log :-> rcons lg (res, d))
   :=
   Do (e <-- read_round;
       send_prep_loop e d;;
-      res <-- receive_prep_loop e;                     
+      res <-- receive_prep_loop e;
       b <-- read_resp_result;
       (if b
        then send_commits e d;;
-            receive_commit_loop e                
+            receive_commit_loop e
        else send_aborts e d;;
-            receive_abort_loop e);; 
+            receive_abort_loop e);;
       ret _ _ b).
 Next Obligation.
 move=>s0/=[e][lg]E0; apply: step.
@@ -867,7 +867,7 @@ case:ifP=>A.
   apply: call_rule=>//_ s6 E6 C6.
   apply: ret_rule=>i6 R6 e' lg' E0'.
   rewrite E0 in E0'; case: (hcancelV _ E0'); first by rewrite validPtUn.
-  + case=>Z1 _; subst e'; move/(hcancelPtV _)=>/=.
+  + case=>Z1 _; subst e'; move/(hcancelPtV _).
   by rewrite validPt (rely_loc' _ R6)=>/(_ is_true_true)=><-.
 do![apply: step]; apply: (gh_ex (g:=lg)).
 apply: call_rule=>_; first by exists res; rewrite has_predC A.
@@ -875,9 +875,9 @@ move=>s5 E5 C5; apply: (gh_ex (g:=(d, lg))).
 apply: call_rule=>//_ s6 E6 C6.
 apply: ret_rule=>i6 R6 e' lg' E0'.
 rewrite E0 in E0'; case: (hcancelV _ E0'); first by rewrite validPtUn.
-- case=>Z1 _; subst e'; move/(hcancelPtV _)=>/=.
+- case=>Z1 _; subst e'; move/(hcancelPtV _).
 by rewrite validPt (rely_loc' _ R6)=>/(_ is_true_true)=><-.
-Qed.                                                     
+Qed.
 
 (**************************************************)
 (*
@@ -896,11 +896,11 @@ TODO: Do something about severe proof duplication!
 (*****************************************************)
 
 Definition coord_loop_spec := forall dts,
-  {(el : nat * Log)}, DHT [cn, W] 
+  {(el : nat * Log)}, DHT [cn, W]
   (fun i =>  loc i = st :-> (el.1, CInit) \+ log :-> el.2,
    fun (_ : unit) m => exists (chs : seq bool),
      loc m = st :-> (el.1 + (size dts), CInit) \+ log :-> (el.2 ++ (seq.zip chs dts))).
-                                               
+
 
 Program Definition coord_loop : coord_loop_spec :=
   fun dts  =>
@@ -910,7 +910,7 @@ Program Definition coord_loop : coord_loop_spec :=
            | [::] => ret _ _ tt
            end)) dts.
 Next Obligation.
-apply:ghC=>i; elim: dts i=>//=[|d ds/= Hi]i1 [e lg] E1 C1. 
+apply:ghC=>i; elim: dts i=>//=[|d ds/= Hi]i1 [e lg] E1 C1.
 - by apply: ret_rule=>i2 R1; exists [::]; rewrite cats0 addn0 (rely_loc' _ R1).
 apply: step; apply: (gh_ex (g:=e)); apply: (gh_ex (g:=lg)).
 apply: call_rule=>//b i2/=E2 C2/=.
@@ -919,8 +919,8 @@ rewrite -[e.+1]addn1 -[(size ds).+1]addn1 addnAC addnA; exists (b :: chs)=>/=.
 by rewrite -cats1 -!catA/=.
 Qed.
 
-Program Definition coordinator_loop_zero (ds : seq data) : 
-  DHT [cn, W] 
+Program Definition coordinator_loop_zero (ds : seq data) :
+  DHT [cn, W]
   (fun i =>  loc i = st :-> (0, CInit) \+ log :-> ([::] : seq (bool * data)),
    fun (_ : unit) m => exists (chs : seq bool),
        loc m = st :-> (size ds, CInit) \+ log :-> (seq.zip chs ds))
